updated invs_dv_next_3

src/proofs/no_slashable_blocks/supporting_lemmas/dv_next_preserves_ind_inv/invs_dv_next_3.dfy
@@ -1,954 +1,1239 @@
-include "../../../../common/commons.dfy"
-include "../../common/attestation_creation_instrumented.dfy"
-include "../../../../specs/consensus/consensus.dfy"
-include "../../../../specs/network/network.dfy"
-include "../../../../specs/dv/dv_attestation_creation.dfy"
-
-include "../../../common/helper_sets_lemmas.dfy"
-include "../../common/common_proofs.dfy"
-include "../../common/dvc_spec_axioms.dfy"
-
-include "../inv.dfy"
-
 include "invs_fnc_1.dfy"
 include "invs_fnc_2.dfy"
+
+include "../../../../common/block_proposer/block_types.dfy"
+include "../../../../common/block_proposer/block_common_functions.dfy"
+include "../../../../common/block_proposer/block_signing_functions.dfy"
+include "../../common/dvc_block_proposer_instrumented.dfy"
+include "../../common/block_dvc_spec_axioms.dfy"
+
+include "../../../../specs/consensus/block_consensus.dfy"
+include "../../../../specs/network/block_network.dfy"
+include "../../../../specs/dv/dv_block_proposer.dfy"
+include "../inv.dfy"
+
+include "../../common/common_proofs.dfy"
+include "../../common/block_dvc_spec_axioms.dfy"
+
+include "../inv.dfy"
+include "../../../common/helper_sets_lemmas.dfy"
+include "../../../common/helper_pred_fcn.dfy"
+include "../../common/common_proofs.dfy"
+
 include "invs_dv_next_1.dfy"
 include "invs_dv_next_2.dfy"
 
 module Invs_DV_Next_3
 {
-    import opened Types 
-    import opened CommonFunctions
-    import opened ConsensusSpec
-    import opened NetworkSpec
-    import opened DVC_Spec
-    import opened DV
-    import opened Att_Inv_With_Empty_Initial_Attestation_Slashing_DB
+    import opened Block_Types
+    import opened Block_Signing_Functions
+    import opened Block_Common_Functions
+    import opened Block_Consensus_Spec
+    import opened Block_Network_Spec
+    import opened DVC_Block_Proposer_Spec_Instr
+    import opened DVC_Block_Proposer_Spec_Axioms
+    import opened Block_Inv_With_Empty_Initial_Block_Slashing_DB
+    import opened DV_Block_Proposer_Spec    
     import opened Fnc_Invs_1
-    import opened Helper_Sets_Lemmas
-    import opened Invs_DV_Next_1
     import opened Fnc_Invs_2
-    import opened DVC_Spec_Axioms
+    import opened Helper_Sets_Lemmas
+    import opened Common_Proofs_For_Block_Proposer
+    import opened Invs_DV_Next_1
     import opened Invs_DV_Next_2
 
-    lemma lem_inv_att_slashing_db_hist_keeps_track_of_only_rcvd_att_duties_dv_next(
-        dv: DVState,
-        event: DV.Event,
-        dv': DVState
-    )    
-    requires NextEventPreCond(dv, event)
-    requires NextEvent(dv, event, dv')    
-    requires inv_consensus_instance_only_for_slot_in_which_dvc_has_rcvd_att_duty(dv)
-    requires inv_att_slashing_db_hist_keeps_track_of_only_rcvd_att_duties(dv)  
-    ensures inv_att_slashing_db_hist_keeps_track_of_only_rcvd_att_duties(dv')
-    {        
-        match event 
-        {
-            case HonestNodeTakingStep(node, nodeEvent, nodeOutputs) =>
-                var dvc := dv.honest_nodes_states[node];
-                var dvc' := dv'.honest_nodes_states[node];                
-                
-                match nodeEvent
-                {
-                    case ServeAttestationDuty(attestation_duty) =>   
-                        assert inv_consensus_instance_only_for_slot_in_which_dvc_has_rcvd_att_duty_body(dvc);   
-                        assert inv_att_slashing_db_hist_keeps_track_of_only_rcvd_att_duties_body(dvc);                                           
-                        lem_inv_att_slashing_db_hist_keeps_track_of_only_rcvd_att_duties_body_f_serve_attestation_duty(dvc, attestation_duty, dvc');
-                        assert inv_att_slashing_db_hist_keeps_track_of_only_rcvd_att_duties_body(dvc');
-                        
-                    case AttConsensusDecided(id, decided_attestation_data) => 
-                        lem_inv_att_slashing_db_hist_keeps_track_of_only_rcvd_att_duties_body_f_att_consensus_decided(dvc, id, decided_attestation_data, dvc');
-                        assert inv_att_slashing_db_hist_keeps_track_of_only_rcvd_att_duties_body(dvc');
-                        
-                    case ReceivedAttestationShare(attestation_share) =>                         
-                        lem_inv_att_slashing_db_hist_keeps_track_of_only_rcvd_att_duties_body_f_listen_for_attestation_shares(dvc, attestation_share, dvc');
-                        assert inv_att_slashing_db_hist_keeps_track_of_only_rcvd_att_duties_body(dvc');
-                       
-                    case ImportedNewBlock(block) => 
-                        var dvc_mod := f_add_block_to_bn(dvc, block);
-                        lem_inv_att_slashing_db_hist_keeps_track_of_only_rcvd_att_duties_body_f_add_block_to_bn(dvc, block, dvc_mod);
-                        assert inv_att_slashing_db_hist_keeps_track_of_only_rcvd_att_duties_body(dvc_mod);
-                        lem_inv_att_slashing_db_hist_keeps_track_of_only_rcvd_att_duties_body_f_listen_for_new_imported_blocks(dvc_mod, block, dvc');                        
-                        assert inv_att_slashing_db_hist_keeps_track_of_only_rcvd_att_duties_body(dvc');
-
-                    case ResendAttestationShares =>                                                                      
-
-                    case NoEvent => 
-                        
-                }
-                
-            case AdversaryTakingStep(node, new_attestation_shares_sent, messagesReceivedByTheNode) =>
-                
-        }   
-    }
-
-    lemma lem_inv_exists_db_in_att_slashing_db_hist_and_duty_for_every_validity_predicate_dv_next(
-        dv: DVState,
-        event: DV.Event,
-        dv': DVState
-    )    
-    requires NextEventPreCond(dv, event)
-    requires NextEvent(dv, event, dv')    
-    requires inv_consensus_instances_only_for_rcvd_duties(dv)
-    requires inv_exists_db_in_att_slashing_db_hist_and_duty_for_every_validity_predicate(dv)  
-    ensures inv_exists_db_in_att_slashing_db_hist_and_duty_for_every_validity_predicate(dv')
-    {        
-        match event 
-        {
-            case HonestNodeTakingStep(node, nodeEvent, nodeOutputs) =>
-                var dvc := dv.honest_nodes_states[node];
-                var dvc' := dv'.honest_nodes_states[node];                
-                
-                match nodeEvent
-                {
-                    case ServeAttestationDuty(attestation_duty) =>   
-                        
-                        assert inv_consensus_instances_only_for_rcvd_duties_body(dvc);   
-                        assert inv_exists_db_in_att_slashing_db_hist_and_duty_for_every_validity_predicate_body(dvc);                                           
-                        lem_inv_exists_db_in_att_slashing_db_hist_and_duty_for_every_validity_predicate_body_f_serve_attestation_duty(dvc, attestation_duty, dvc');
-                        assert inv_exists_db_in_att_slashing_db_hist_and_duty_for_every_validity_predicate_body(dvc');
-                        
-                    case AttConsensusDecided(id, decided_attestation_data) => 
-                        lem_inv_exists_db_in_att_slashing_db_hist_and_duty_for_every_validity_predicate_body_f_att_consensus_decided(dvc, id, decided_attestation_data, dvc');
-                        assert inv_exists_db_in_att_slashing_db_hist_and_duty_for_every_validity_predicate_body(dvc');
-                        
-                    case ReceivedAttestationShare(attestation_share) =>                         
-                        lem_inv_exists_db_in_att_slashing_db_hist_and_duty_for_every_validity_predicate_body_f_listen_for_attestation_shares(dvc, attestation_share, dvc');
-                        assert inv_exists_db_in_att_slashing_db_hist_and_duty_for_every_validity_predicate_body(dvc');
-                       
-                    case ImportedNewBlock(block) => 
-                        var dvc_mod := f_add_block_to_bn(dvc, block);
-                        lem_inv_exists_db_in_att_slashing_db_hist_and_duty_for_every_validity_predicate_body_f_add_block_to_bn(dvc, block, dvc_mod);
-                        assert inv_exists_db_in_att_slashing_db_hist_and_duty_for_every_validity_predicate_body(dvc_mod);
-                        lem_inv_exists_db_in_att_slashing_db_hist_and_duty_for_every_validity_predicate_body_f_listen_for_new_imported_blocks(dvc_mod, block, dvc');                        
-                        assert inv_exists_db_in_att_slashing_db_hist_and_duty_for_every_validity_predicate_body(dvc');
-
-                    case ResendAttestationShares =>                                                                      
-
-                    case NoEvent => 
-                        
-                }
-                
-            case AdversaryTakingStep(node, new_attestation_shares_sent, messagesReceivedByTheNode) =>
-                
-        }   
-    }
-
-    lemma lem_inv_current_validity_predicate_for_slot_k_is_stored_in_att_slashing_db_hist_k_dv_next(
-        dv: DVState,
-        event: DV.Event,
-        dv': DVState
-    )    
-    requires NextEventPreCond(dv, event)
-    requires NextEvent(dv, event, dv')    
-    requires inv_consensus_instance_only_for_slot_in_which_dvc_has_rcvd_att_duty(dv)
-    requires inv_current_validity_predicate_for_slot_k_is_stored_in_att_slashing_db_hist_k(dv)  
-    ensures inv_current_validity_predicate_for_slot_k_is_stored_in_att_slashing_db_hist_k(dv')
-    {        
-        match event 
-        {
-            case HonestNodeTakingStep(node, nodeEvent, nodeOutputs) =>
-                var dvc := dv.honest_nodes_states[node];
-                var dvc' := dv'.honest_nodes_states[node];                
-                
-                match nodeEvent
-                {
-                    case ServeAttestationDuty(attestation_duty) =>   
-                        
-                        assert inv_consensus_instance_only_for_slot_in_which_dvc_has_rcvd_att_duty_body(dvc);   
-                        assert inv_current_validity_predicate_for_slot_k_is_stored_in_att_slashing_db_hist_k_body(dvc);                                           
-                        lem_inv_current_validity_predicate_for_slot_k_is_stored_in_att_slashing_db_hist_k_body_f_serve_attestation_duty(dvc, attestation_duty, dvc');
-                        assert inv_current_validity_predicate_for_slot_k_is_stored_in_att_slashing_db_hist_k_body(dvc');
-                        
-                    case AttConsensusDecided(id, decided_attestation_data) => 
-                        lem_inv_current_validity_predicate_for_slot_k_is_stored_in_att_slashing_db_hist_k_body_f_att_consensus_decided(dvc, id, decided_attestation_data, dvc');
-                        assert inv_current_validity_predicate_for_slot_k_is_stored_in_att_slashing_db_hist_k_body(dvc');
-                        
-                    case ReceivedAttestationShare(attestation_share) =>                         
-                        lem_inv_current_validity_predicate_for_slot_k_is_stored_in_att_slashing_db_hist_k_body_f_listen_for_attestation_shares(dvc, attestation_share, dvc');
-                        assert inv_current_validity_predicate_for_slot_k_is_stored_in_att_slashing_db_hist_k_body(dvc');
-                       
-                    case ImportedNewBlock(block) => 
-                        var dvc_mod := f_add_block_to_bn(dvc, block);
-                        lem_inv_current_validity_predicate_for_slot_k_is_stored_in_att_slashing_db_hist_k_body_f_add_block_to_bn(dvc, block, dvc_mod);
-                        assert inv_current_validity_predicate_for_slot_k_is_stored_in_att_slashing_db_hist_k_body(dvc_mod);
-                        lem_inv_current_validity_predicate_for_slot_k_is_stored_in_att_slashing_db_hist_k_body_f_listen_for_new_imported_blocks(dvc_mod, block, dvc');                        
-                        assert inv_current_validity_predicate_for_slot_k_is_stored_in_att_slashing_db_hist_k_body(dvc');
-
-                    case ResendAttestationShares =>                                                                      
-
-                    case NoEvent => 
-                        
-                }
-                
-            case AdversaryTakingStep(node, new_attestation_shares_sent, messagesReceivedByTheNode) =>
-                
-        }   
-    }
-
-    lemma lem_inv_monotonic_att_slashing_db_dv_next(
-        dv: DVState,
-        event: DV.Event,
-        dv': DVState
-    )    
-    requires NextEventPreCond(dv, event)
-    requires NextEvent(dv, event, dv')    
-    ensures inv_monotonic_att_slashing_db(dv, event, dv')
-    {        
-        match event 
-        {
-            case HonestNodeTakingStep(node, nodeEvent, nodeOutputs) =>
-                var dvc := dv.honest_nodes_states[node];
-                var dvc' := dv'.honest_nodes_states[node];                
-                
-                match nodeEvent
-                {
-                    case ServeAttestationDuty(attestation_duty) =>   
-                        lem_inv_monotonic_att_slashing_db_body_f_serve_attestation_duty(dvc, attestation_duty, dvc');
-                        assert inv_monotonic_att_slashing_db_body(dvc, dvc');
-                        
-                    case AttConsensusDecided(id, decided_attestation_data) => 
-                        lem_inv_monotonic_att_slashing_db_body_f_att_consensus_decided(dvc, id, decided_attestation_data, dvc');
-                        assert inv_monotonic_att_slashing_db_body(dvc, dvc');
-                        
-                    case ReceivedAttestationShare(attestation_share) =>                         
-                        lem_inv_monotonic_att_slashing_db_body_f_listen_for_attestation_shares(dvc, attestation_share, dvc');
-                        assert inv_monotonic_att_slashing_db_body(dvc, dvc');
-                       
-                    case ImportedNewBlock(block) => 
-                        var dvc_mod := f_add_block_to_bn(dvc, block);
-                        lem_inv_monotonic_att_slashing_db_body_f_add_block_to_bn(dvc, block, dvc_mod);
-                        assert inv_monotonic_att_slashing_db_body(dvc, dvc_mod);
-                        lem_inv_monotonic_att_slashing_db_body_f_listen_for_new_imported_blocks(dvc_mod, block, dvc');                        
-                        assert inv_monotonic_att_slashing_db_body(dvc_mod, dvc');
-
-                    case ResendAttestationShares =>                                                                      
-
-                    case NoEvent => 
-                        
-                }
-                
-            case AdversaryTakingStep(node, new_attestation_shares_sent, messagesReceivedByTheNode) =>
-                
-        }   
-    }
-
-    lemma lem_inv_every_db_in_att_slashing_db_hist_is_subset_of_att_slashing_db_dv_next(
-        dv: DVState,
-        event: DV.Event,
-        dv': DVState
-    )    
-    requires NextEventPreCond(dv, event)
-    requires NextEvent(dv, event, dv')    
-    requires inv_consensus_instances_only_for_rcvd_duties(dv)
-    requires inv_every_db_in_att_slashing_db_hist_is_subset_of_att_slashing_db(dv)  
-    ensures inv_every_db_in_att_slashing_db_hist_is_subset_of_att_slashing_db(dv')
-    {        
-        match event 
-        {
-            case HonestNodeTakingStep(node, nodeEvent, nodeOutputs) =>
-                var dvc := dv.honest_nodes_states[node];
-                var dvc' := dv'.honest_nodes_states[node];                
-                
-                match nodeEvent
-                {
-                    case ServeAttestationDuty(attestation_duty) =>   
-                        
-                        assert inv_consensus_instances_only_for_rcvd_duties_body(dvc);   
-                        assert inv_every_db_in_att_slashing_db_hist_is_subset_of_att_slashing_db_body(dvc);                                           
-                        lem_inv_every_db_in_att_slashing_db_hist_is_subset_of_att_slashing_db_body_f_serve_attestation_duty(dvc, attestation_duty, dvc');
-                        assert inv_every_db_in_att_slashing_db_hist_is_subset_of_att_slashing_db_body(dvc');
-                        
-                    case AttConsensusDecided(id, decided_attestation_data) => 
-                        lem_inv_every_db_in_att_slashing_db_hist_is_subset_of_att_slashing_db_body_f_att_consensus_decided(dvc, id, decided_attestation_data, dvc');
-                        assert inv_every_db_in_att_slashing_db_hist_is_subset_of_att_slashing_db_body(dvc');
-                        
-                    case ReceivedAttestationShare(attestation_share) =>                         
-                        lem_inv_every_db_in_att_slashing_db_hist_is_subset_of_att_slashing_db_body_f_listen_for_attestation_shares(dvc, attestation_share, dvc');
-                        assert inv_every_db_in_att_slashing_db_hist_is_subset_of_att_slashing_db_body(dvc');
-                       
-                    case ImportedNewBlock(block) => 
-                        var dvc_mod := f_add_block_to_bn(dvc, block);
-                        lem_inv_every_db_in_att_slashing_db_hist_is_subset_of_att_slashing_db_body_f_add_block_to_bn(dvc, block, dvc_mod);
-                        assert inv_every_db_in_att_slashing_db_hist_is_subset_of_att_slashing_db_body(dvc_mod);
-                        lem_inv_every_db_in_att_slashing_db_hist_is_subset_of_att_slashing_db_body_f_listen_for_new_imported_blocks(dvc_mod, block, dvc');                        
-                        assert inv_every_db_in_att_slashing_db_hist_is_subset_of_att_slashing_db_body(dvc');
-
-                    case ResendAttestationShares =>                                                                      
-
-                    case NoEvent => 
-                        
-                }
-                
-            case AdversaryTakingStep(node, new_attestation_shares_sent, messagesReceivedByTheNode) =>
-                
-        }   
-    }
-
-    lemma lem_inv_monotonic_att_slashing_db_hist_dv_next(
-        dv: DVState,
-        event: DV.Event,
-        dv': DVState
-    )    
-    requires NextEventPreCond(dv, event)
-    requires NextEvent(dv, event, dv')    
-    ensures inv_monotonic_att_slashing_db_hist(dv, event, dv')
-    {        
-        match event 
-        {
-            case HonestNodeTakingStep(node, nodeEvent, nodeOutputs) =>
-                var dvc := dv.honest_nodes_states[node];
-                var dvc' := dv'.honest_nodes_states[node];                
-                
-                match nodeEvent
-                {
-                    case ServeAttestationDuty(attestation_duty) =>   
-                        lem_inv_monotonic_att_slashing_db_hist_body_f_serve_attestation_duty(dvc, attestation_duty, dvc');
-                        assert inv_monotonic_att_slashing_db_hist_body(dvc, dvc');
-                        
-                    case AttConsensusDecided(id, decided_attestation_data) => 
-                        lem_inv_monotonic_att_slashing_db_hist_body_f_att_consensus_decided(dvc, id, decided_attestation_data, dvc');
-                        assert inv_monotonic_att_slashing_db_hist_body(dvc, dvc');
-                        
-                    case ReceivedAttestationShare(attestation_share) =>                         
-                        lem_inv_monotonic_att_slashing_db_hist_body_f_listen_for_attestation_shares(dvc, attestation_share, dvc');
-                        assert inv_monotonic_att_slashing_db_hist_body(dvc, dvc');
-                       
-                    case ImportedNewBlock(block) => 
-                        var dvc_mod := f_add_block_to_bn(dvc, block);
-                        lem_inv_monotonic_att_slashing_db_hist_body_f_add_block_to_bn(dvc, block, dvc_mod);
-                        assert inv_monotonic_att_slashing_db_hist_body(dvc, dvc_mod);
-                        lem_inv_monotonic_att_slashing_db_hist_body_f_listen_for_new_imported_blocks(dvc_mod, block, dvc');                        
-                        assert inv_monotonic_att_slashing_db_hist_body(dvc_mod, dvc');
-
-                    case ResendAttestationShares =>                                                                      
-
-                    case NoEvent => 
-                        
-                }
-                
-            case AdversaryTakingStep(node, new_attestation_shares_sent, messagesReceivedByTheNode) =>
-                
-        }   
-    }
-
-    lemma lem_inv_active_attn_consensus_instances_are_tracked_in_att_slashing_db_hist_dv_next(
-        dv: DVState,
-        event: DV.Event,
-        dv': DVState
-    )    
-    requires NextEventPreCond(dv, event)
-    requires NextEvent(dv, event, dv')    
-    requires inv_active_attn_consensus_instances_are_tracked_in_att_slashing_db_hist(dv)
-    ensures inv_active_attn_consensus_instances_are_tracked_in_att_slashing_db_hist(dv')
-    {        
-        match event 
-        {
-            case HonestNodeTakingStep(node, nodeEvent, nodeOutputs) =>
-                var dvc := dv.honest_nodes_states[node];
-                var dvc' := dv'.honest_nodes_states[node];                
-                
-                match nodeEvent
-                {
-                    case ServeAttestationDuty(attestation_duty) =>   
-                        lem_inv_active_attn_consensus_instances_are_tracked_in_att_slashing_db_hist_body_f_serve_attestation_duty(dvc, attestation_duty, dvc');
-                        assert inv_active_attn_consensus_instances_are_tracked_in_att_slashing_db_hist_body(dvc');
-                        
-                    case AttConsensusDecided(id, decided_attestation_data) => 
-                        lem_inv_active_attn_consensus_instances_are_tracked_in_att_slashing_db_hist_body_f_att_consensus_decided(dvc, id, decided_attestation_data, dvc');
-                        assert inv_active_attn_consensus_instances_are_tracked_in_att_slashing_db_hist_body(dvc');
-                        
-                    case ReceivedAttestationShare(attestation_share) =>                         
-                        lem_inv_active_attn_consensus_instances_are_tracked_in_att_slashing_db_hist_body_f_listen_for_attestation_shares(dvc, attestation_share, dvc');
-                        assert inv_active_attn_consensus_instances_are_tracked_in_att_slashing_db_hist_body(dvc');
-                       
-                    case ImportedNewBlock(block) => 
-                        var dvc_mod := f_add_block_to_bn(dvc, block);
-                        lem_inv_active_attn_consensus_instances_are_tracked_in_att_slashing_db_hist_body_f_add_block_to_bn(dvc, block, dvc_mod);
-                        assert inv_active_attn_consensus_instances_are_tracked_in_att_slashing_db_hist_body(dvc_mod);
-                        lem_inv_active_attn_consensus_instances_are_tracked_in_att_slashing_db_hist_body_f_listen_for_new_imported_blocks(dvc_mod, block, dvc');                        
-                        assert inv_active_attn_consensus_instances_are_tracked_in_att_slashing_db_hist_body(dvc');
-
-                    case ResendAttestationShares =>                                                                      
-
-                    case NoEvent => 
-                        
-                }
-                
-            case AdversaryTakingStep(node, new_attestation_shares_sent, messagesReceivedByTheNode) =>
-                
-        }   
-    }
-
-    lemma lem_inv_construct_signed_attestation_signature_assumptions_helper_dv_next(
-        dv: DVState,
-        event: DV.Event,
-        dv': DVState
-    )    
-    requires NextEventPreCond(dv, event)
-    requires NextEvent(dv, event, dv')    
-    requires inv_construct_signed_attestation_signature_assumptions_helper(dv)
-    ensures inv_construct_signed_attestation_signature_assumptions_helper(dv')    
+    lemma f_inv_sent_validity_predicate_is_based_on_rcvd_proposer_duty_and_slashing_db_and_randao_reveal_get_s_w_honest_node_states_updated(
+        s: DVState,
+        node: BLSPubkey,
+        nodeEvent: Block_Types.Event
+    ) returns (s_w_honest_node_states_updated: DVState)
+    requires node in s.honest_nodes_states
+    ensures s_w_honest_node_states_updated == add_block_to_bn_with_event(s, node, nodeEvent)
+    ensures s_w_honest_node_states_updated == s.(honest_nodes_states := s_w_honest_node_states_updated.honest_nodes_states)
+    ensures s_w_honest_node_states_updated.honest_nodes_states == s.honest_nodes_states[node := s_w_honest_node_states_updated.honest_nodes_states[node]]
+    ensures s_w_honest_node_states_updated.honest_nodes_states[node] == s.honest_nodes_states[node].(bn := s_w_honest_node_states_updated.honest_nodes_states[node].bn)
+    ensures s_w_honest_node_states_updated.consensus_instances_on_beacon_block.Keys == s.consensus_instances_on_beacon_block.Keys
     {
-        assert dv.construct_signed_attestation_signature == dv'.construct_signed_attestation_signature;
+        s_w_honest_node_states_updated :=
+        if nodeEvent.ImportedNewBlock? then
+            s.(
+                honest_nodes_states := s.honest_nodes_states[node := f_add_block_to_bn(s.honest_nodes_states[node], nodeEvent.block)]
+            )
+        else
+            s           
+        ;         
     }
 
+    lemma lem_inv_sent_validity_predicate_is_based_on_rcvd_proposer_duty_and_slashing_db_and_randao_reveal_get_s_w_honest_node_states_updated_2(
+        s: DVState,
+        node: BLSPubkey,
+        nodeEvent: Block_Types.Event,
+        node': BLSPubkey,
+        s_w_honest_node_states_updated: DVState
+    )
+    requires node in s.honest_nodes_states
+    requires node' in s.honest_nodes_states
+    requires s_w_honest_node_states_updated == add_block_to_bn_with_event(s, node, nodeEvent)
+    ensures s_w_honest_node_states_updated.honest_nodes_states[node'].block_consensus_engine_state == s.honest_nodes_states[node'].block_consensus_engine_state
+    {
+    }
 
-
-    lemma lem_inv_attestation_shares_to_broadcast_are_sent_messages_dv_next(
-        dv: DVState,
-        event: DV.Event,
-        dv': DVState
-    )       
-    requires NextEventPreCond(dv, event)
-    requires NextEvent(dv, event, dv')  
-    requires inv_quorum_constraints(dv)
-    requires inv_unchanged_paras_of_consensus_instances(dv)
-    requires inv_only_dv_construct_signed_attestation_signature(dv)
-    requires same_honest_nodes_in_dv_and_ci(dv)    
-    requires inv_decided_value_of_consensus_instance_is_decided_by_quorum(dv)    
-    requires inv_sent_validity_predicate_is_based_on_rcvd_att_duty_and_slashing_db(dv)
-    requires inv_sent_validity_predicate_is_based_on_rcvd_att_duty_and_slashing_db_for_dv(dv)      
-    requires inv_decided_value_of_consensus_instance_of_slot_k_is_for_slot_k(dv)       
-    requires inv_attestation_shares_to_broadcast_are_sent_messages(dv)    
-    ensures inv_attestation_shares_to_broadcast_are_sent_messages(dv')
-    {   
-        lem_inv_quorum_constraints_dv_next(dv, event, dv');
-        lem_inv_unchanged_paras_of_consensus_instances_dv_next(dv, event, dv');
-        lem_inv_only_dv_construct_signed_attestation_signature_dv_next(dv, event, dv');
-
-        assert && inv_quorum_constraints(dv')
-               && inv_unchanged_paras_of_consensus_instances(dv')
-               && inv_only_dv_construct_signed_attestation_signature(dv');
-        
-
-        match event 
+    lemma lem_inv_sent_validity_predicate_is_based_on_rcvd_proposer_duty_and_slashing_db_and_randao_reveal_helper(
+        s: DVState,
+        event: DV_Block_Proposer_Spec.Event,
+        s': DVState,
+        cid: Slot,
+        hn: BLSPubkey,
+        vp: BeaconBlock -> bool
+    ) returns (proposer_duty: ProposerDuty, block_slashing_db: set<SlashingDBBlock>, randao_reveal: BLSSignature)
+    requires NextEventPreCond(s, event)
+    requires NextEvent(s, event, s')
+    requires event.HonestNodeTakingStep?
+    requires inv_quorum_constraints(s)
+    requires inv_unchanged_paras_of_consensus_instances(s)
+    requires inv_only_dv_construct_complete_signed_block(s)
+    requires && hn in s'.consensus_instances_on_beacon_block[cid].honest_nodes_validity_functions.Keys
+             && vp in s'.consensus_instances_on_beacon_block[cid].honest_nodes_validity_functions[hn]    
+    requires inv_sent_validity_predicate_is_based_on_rcvd_proposer_duty_and_slashing_db_and_randao_reveal(s)
+    requires inv_sent_validity_predicate_is_based_on_rcvd_proposer_duty_and_slashing_db_and_randao_reveal_for_dv(s)
+    ensures inv_sent_validity_predicate_is_based_on_rcvd_proposer_duty_and_slashing_db_and_randao_reveal_body(
+                cid, 
+                proposer_duty, 
+                block_slashing_db, 
+                randao_reveal, 
+                vp);
+    {
+        assert s.block_share_network.allMessagesSent <= s'.block_share_network.allMessagesSent;
+        match event
         {
             case HonestNodeTakingStep(node, nodeEvent, nodeOutputs) =>
-                var dvc := dv.honest_nodes_states[node];
-                var dvc' := dv'.honest_nodes_states[node];
-                assert && dvc.peers == dvc'.peers
-                       && |dvc.peers| > 0 ;
+                var s_node := s.honest_nodes_states[node];
+                var s'_node := s'.honest_nodes_states[node];
 
-                match nodeEvent
-                {
-                    case ServeAttestationDuty(att_duty) =>     
-                        lem_inv_attestation_shares_to_broadcast_are_sent_messages_f_serve_attestation_duty(dvc, att_duty, dvc');                        
-                        
-                    case AttConsensusDecided(id, decided_attestation_data) => 
-                        var att_network := dv.att_network;
-                        var att_network' := dv'.att_network;
-                        if id == decided_attestation_data.slot
-                        {
-                            lem_inv_attestation_shares_to_broadcast_are_sent_messages_f_att_consensus_decided(dvc, id, decided_attestation_data, dvc', nodeOutputs);   
-                            assert att_network'.allMessagesSent
-                                        == att_network.allMessagesSent + getMessagesFromMessagesWithRecipient(nodeOutputs.att_shares_sent);               
-                        }
-                                                
-                    case ReceivedAttestationShare(attestation_share) =>                         
-                        lem_inv_attestation_shares_to_broadcast_are_sent_messages_f_listen_for_attestation_shares(dvc, attestation_share, dvc');                                                
+                var s_w_honest_node_states_updated :=
+                    f_inv_sent_validity_predicate_is_based_on_rcvd_proposer_duty_and_slashing_db_and_randao_reveal_get_s_w_honest_node_states_updated(s, node, nodeEvent);
 
-                    case ImportedNewBlock(block) => 
-                        var dvc_mod := f_add_block_to_bn(dvc, block);
-                        lem_inv_attestation_shares_to_broadcast_are_sent_messages_add_block_to_bn(dvc, block, dvc_mod);
-                        lem_inv_attestation_shares_to_broadcast_are_sent_messages_f_listen_for_new_imported_blocks(dvc_mod, block, dvc');                                                
-                                                
-                    case ResendAttestationShares =>                         
-                        lem_inv_attestation_shares_to_broadcast_are_sent_messages_f_resend_attestation_share(dvc, dvc');
+                assert s_w_honest_node_states_updated.consensus_instances_on_beacon_block == s.consensus_instances_on_beacon_block;
 
-                    case NoEvent => 
-                        
-                }
 
-            case AdversaryTakingStep(node, new_attestation_shares_sent, messagesReceivedByTheNode) =>
-                
-        }        
-    }  
+                var output :=
+                    if nodeEvent.BlockConsensusDecided? && nodeEvent.id == cid then
+                        Some(Decided(node, nodeEvent.decided_beacon_block))
+                    else
+                        None
+                    ;
 
-    // TODO: Rename
-    lemma lem_inv39_dv_next(
-        dv: DVState,
-        event: DV.Event,
-        dv': DVState
-    )       
-    requires NextEventPreCond(dv, event)
-    requires NextEvent(dv, event, dv')  
-    ensures dv.att_network.allMessagesSent <= dv'.att_network.allMessagesSent
-    {}
+                var validityPredicates :=
+                    map n |
+                            && n in s_w_honest_node_states_updated.honest_nodes_states.Keys
+                            && cid in s_w_honest_node_states_updated.honest_nodes_states[n].block_consensus_engine_state.active_consensus_instances_on_beacon_blocks.Keys
+                        ::
+                            s_w_honest_node_states_updated.honest_nodes_states[n].block_consensus_engine_state.active_consensus_instances_on_beacon_blocks[cid].validityPredicate
+                    ;
 
-    lemma lem_inv_rcvd_attn_shares_are_from_sent_messages_dv_next(
-        dv: DVState,
-        event: DV.Event,
-        dv': DVState
-    )       
-    requires NextEventPreCond(dv, event)
-    requires NextEvent(dv, event, dv')  
-    requires inv_all_in_transit_messages_were_sent(dv)
-    requires inv_rcvd_attn_shares_are_from_sent_messages(dv)
-    ensures inv_rcvd_attn_shares_are_from_sent_messages(dv')
-    {        
-        match event 
-        {
-            case HonestNodeTakingStep(node, nodeEvent, nodeOutputs) =>
-                var dvc := dv.honest_nodes_states[node];
-                var dvc' := dv'.honest_nodes_states[node];
-                match nodeEvent
-                {
-                    case ServeAttestationDuty(att_duty) =>     
-                        lem_inv_rcvd_attn_shares_are_from_sent_messages_f_serve_attestation_duty(dvc, att_duty, dvc');                        
-                        
-                    case AttConsensusDecided(id, decided_attestation_data) => 
-                        lem_inv_rcvd_attn_shares_are_from_sent_messages_f_att_consensus_decided(dvc, id, decided_attestation_data, dvc');                        
+                var s_consensus := s_w_honest_node_states_updated.consensus_instances_on_beacon_block[cid];
+                var s'_consensus := s'.consensus_instances_on_beacon_block[cid];
 
-                    case ReceivedAttestationShare(attestation_share) =>    
-                        assert NetworkSpec.Next(dv.att_network, dv'.att_network, node, nodeOutputs.att_shares_sent, {attestation_share});
-                        assert multiset(addReceipientToMessages<AttestationShare>({attestation_share}, node)) <= dv.att_network.messagesInTransit;
-                        assert MessaageWithRecipient(message := attestation_share, receipient := node) in dv.att_network.messagesInTransit;        
-                        assert attestation_share in dv.att_network.allMessagesSent;
-                        assert attestation_share in dv'.att_network.allMessagesSent;
-                        
-                        lem_inv39_dv_next(dv, event, dv');
-                        assert dv.att_network.allMessagesSent <= dv'.att_network.allMessagesSent;
-                        
-                        lem_inv_rcvd_attn_shares_are_from_sent_messages_f_listen_for_attestation_shares(dvc, attestation_share, dvc');  
-
-                        assert dvc' == f_listen_for_attestation_shares(dvc, attestation_share).state;
-
-                        var k := (attestation_share.data, attestation_share.aggregation_bits);
-                        forall i, j | && i in dvc'.rcvd_attestation_shares.Keys 
-                                      && j in dvc'.rcvd_attestation_shares[i].Keys
-                        ensures dvc'.rcvd_attestation_shares[i][j] <= dv'.att_network.allMessagesSent;
-                        {
-                            if ( || i != attestation_share.data.slot
-                                 || j != k
-                               )
-                            {             
-                                lem_inv_rcvd_attn_shares_are_from_sent_messages_f_listen_for_attestation_shares_domain(
-                                    dvc,
-                                    attestation_share,
-                                    dvc'
-                                );
-                                assert && i in dvc.rcvd_attestation_shares.Keys 
-                                       && j in dvc.rcvd_attestation_shares[i].Keys;
-                                assert dvc'.rcvd_attestation_shares[i][j] <= dvc.rcvd_attestation_shares[i][j];                                
-                                assert dvc.rcvd_attestation_shares[i][j] <= dv.att_network.allMessagesSent;
-                                lemmaSubsetOfSubset(
-                                    dvc'.rcvd_attestation_shares[i][j],
-                                    dvc.rcvd_attestation_shares[i][j],
-                                    dv.att_network.allMessagesSent
-                                );
-                                assert dv.att_network.allMessagesSent <= dv'.att_network.allMessagesSent;
-                                lemmaSubsetOfSubset(
-                                    dvc'.rcvd_attestation_shares[i][j],                                    
-                                    dv.att_network.allMessagesSent,
-                                    dv'.att_network.allMessagesSent
-                                );
-                                assert dvc'.rcvd_attestation_shares[i][j] <= dv'.att_network.allMessagesSent;
-                            }
-                            else
-                            {
-                                if  && i == attestation_share.data.slot
-                                    && j == k
-                                    && ( || i !in dvc.rcvd_attestation_shares.Keys
-                                         || j !in dvc.rcvd_attestation_shares[i].Keys
-                                       )                                       
-                                {
-                                    
-                                    assert dvc'.rcvd_attestation_shares[i][j] <= {attestation_share};
-                                    
-                                    
-                                    assert attestation_share in dv'.att_network.allMessagesSent;                                    
-                                    lemmaFromMemberToSingletonSet(attestation_share, dv'.att_network.allMessagesSent);
-                                    assert {attestation_share} <= dv'.att_network.allMessagesSent;
-
-                                    lemmaSubsetOfSubset(
-                                            dvc'.rcvd_attestation_shares[i][j],
-                                            {attestation_share},
-                                            dv'.att_network.allMessagesSent
-                                        );
-                                    assert dvc'.rcvd_attestation_shares[i][j] <= dv'.att_network.allMessagesSent;                                     
-                                    
-                                }
-                                else
-                                {
-                                    assert  && i == attestation_share.data.slot
-                                            && j == k
-                                            && i in dvc.rcvd_attestation_shares.Keys 
-                                            && j in dvc.rcvd_attestation_shares[i].Keys;
-
-                                    
-                                    assert dvc'.rcvd_attestation_shares[i][j] 
-                                                <= dvc.rcvd_attestation_shares[i][j] + {attestation_share}; 
-
-                                    assert dvc.rcvd_attestation_shares[i][j] 
-                                                <= dv.att_network.allMessagesSent;                                                
-                                    assert dv.att_network.allMessagesSent <= dv'.att_network.allMessagesSent;      
-                                    lemmaSubsetOfSubset(
-                                        dvc.rcvd_attestation_shares[i][j],
-                                        dv.att_network.allMessagesSent,
-                                        dv'.att_network.allMessagesSent);                                    
-                                    assert dvc.rcvd_attestation_shares[i][j] 
-                                                <= dv'.att_network.allMessagesSent;
-
-                                    assert attestation_share in dv'.att_network.allMessagesSent;                                    
-                                    lemmaFromMemberToSingletonSet(attestation_share, dv'.att_network.allMessagesSent);
-                                    assert {attestation_share} <= dv'.att_network.allMessagesSent;
-
-                                    lemmaUnionOfSubsets(dvc.rcvd_attestation_shares[i][j], {attestation_share}, dv'.att_network.allMessagesSent);                                    
-                                    assert dvc.rcvd_attestation_shares[i][j] + {attestation_share}
-                                                <= dv'.att_network.allMessagesSent;
-
-                                    lemmaSubsetOfSubset(
-                                        dvc'.rcvd_attestation_shares[i][j],
-                                        dvc.rcvd_attestation_shares[i][j] + {attestation_share},
-                                        dv'.att_network.allMessagesSent);
-                                    
-                                    assert dvc'.rcvd_attestation_shares[i][j] <= dv'.att_network.allMessagesSent;                                                                         
-                                }
-                            }
-                        }
-                        assert inv_rcvd_attn_shares_are_from_sent_messages(dv');
-
-                    case ImportedNewBlock(block) => 
-                        var dvc_mod := f_add_block_to_bn(dvc, block);
-                        lem_inv_rcvd_attn_shares_are_from_sent_messages_f_add_block_to_bn(dvc, block, dvc_mod);
-                        lem_inv_rcvd_attn_shares_are_from_sent_messages_f_listen_for_new_imported_blocks(dvc_mod, block, dvc');                                                
-                                                
-                    case ResendAttestationShares =>                         
-                        lem_inv_rcvd_attn_shares_are_from_sent_messages_f_resend_attestation_share(dvc, dvc');
-
-                    case NoEvent => 
-                        
-                }
-
-            case AdversaryTakingStep(node, new_attestation_shares_sent, messagesReceivedByTheNode) =>
-                
-        }        
-    }  
-
-     
-
-    lemma lem_inv_rcvd_att_duty_is_from_dv_seq_for_rcvd_att_duty_dv_next(
-        dv: DVState,
-        event: DV.Event,
-        dv': DVState
-    )    
-    requires NextEventPreCond(dv, event)
-    requires NextEvent(dv, event, dv')  
-    requires inv_rcvd_att_duty_is_from_dv_seq_for_rcvd_att_duty(dv)
-    ensures inv_rcvd_att_duty_is_from_dv_seq_for_rcvd_att_duty(dv')
-    {  
-        assert pred_unchanged_dvn_seq_of_att_duties(dv, dv');
-
-        match event 
-        {
-            case HonestNodeTakingStep(node, nodeEvent, nodeOutputs) =>
-                var dvc := dv.honest_nodes_states[node];
-                var dvc' := dv'.honest_nodes_states[node];
-                match nodeEvent
-                {
-                    case ServeAttestationDuty(attestation_duty) =>    
-                        assert  dv'.index_next_attestation_duty_to_be_served 
-                                ==
-                                dv.index_next_attestation_duty_to_be_served + 1;
-                        assert  inv_rcvd_att_duty_is_from_dv_seq_for_rcvd_att_duty_body_body(                
-                                    attestation_duty, 
-                                    node, 
-                                    dv'.sequence_attestation_duties_to_be_served,
-                                    dv'.index_next_attestation_duty_to_be_served
-                                );
-                        lem_inv_rcvd_att_duty_is_from_dv_seq_for_rcvd_att_duty_body_f_serve_attestation_duty( 
-                                dvc,
-                                attestation_duty,                                
-                                dvc',
-                                node,
-                                dv'.sequence_attestation_duties_to_be_served,    
-                                dv'.index_next_attestation_duty_to_be_served 
-                            );
-                        assert inv_rcvd_att_duty_is_from_dv_seq_for_rcvd_att_duty(dv');    
-
-                    case AttConsensusDecided(id, decided_attestation_data) => 
-                        lem_inv_rcvd_att_duty_is_from_dv_seq_for_rcvd_att_duty_body_f_att_consensus_decided(
-                                dvc,
-                                id,
-                                decided_attestation_data,
-                                dvc',
-                                node,
-                                dv'.sequence_attestation_duties_to_be_served,    
-                                dv'.index_next_attestation_duty_to_be_served
-                            );
-                        assert inv_rcvd_att_duty_is_from_dv_seq_for_rcvd_att_duty(dv');    
-
-                    case ReceivedAttestationShare(attestation_share) =>   
-                        lem_inv_rcvd_att_duty_is_from_dv_seq_for_rcvd_att_duty_body_f_listen_for_attestation_shares(
-                                dvc,
-                                attestation_share,
-                                dvc',
-                                node,
-                                dv'.sequence_attestation_duties_to_be_served,    
-                                dv'.index_next_attestation_duty_to_be_served
-                            );      
-                        assert inv_rcvd_att_duty_is_from_dv_seq_for_rcvd_att_duty(dv');                
-   
-                    case ImportedNewBlock(block) => 
-                        var dvc := f_add_block_to_bn(dvc, nodeEvent.block);
-                        lem_inv_rcvd_att_duty_is_from_dv_seq_for_rcvd_att_duty_body_f_listen_for_new_imported_blocks(
-                            dvc,
-                            block,
-                            dvc',
-                            node,
-                            dv'.sequence_attestation_duties_to_be_served,    
-                            dv'.index_next_attestation_duty_to_be_served
+                assert  Block_Consensus_Spec.Next(
+                            s_consensus,
+                            validityPredicates,
+                            s'_consensus,
+                            output
                         );
-                        assert inv_rcvd_att_duty_is_from_dv_seq_for_rcvd_att_duty(dv');
-                                          
-                    case ResendAttestationShares =>  
-                        assert inv_rcvd_att_duty_is_from_dv_seq_for_rcvd_att_duty(dv');                       
-                        
-                    case NoEvent => 
-                        assert inv_rcvd_att_duty_is_from_dv_seq_for_rcvd_att_duty(dv');        
-                        
+
+                if  && hn in s_consensus.honest_nodes_validity_functions.Keys  
+                    && vp in s_consensus.honest_nodes_validity_functions[hn]
+                {
+                    assert vp in s'_consensus.honest_nodes_validity_functions[hn];
+
+                    proposer_duty, block_slashing_db, randao_reveal :| inv_sent_validity_predicate_is_based_on_rcvd_proposer_duty_and_slashing_db_and_randao_reveal_body(cid, proposer_duty, block_slashing_db, randao_reveal, vp);
+                }
+                else
+                {
+                    assert vp in validityPredicates.Values;
+
+                    var vpn :| vpn in validityPredicates.Keys && validityPredicates[vpn] == vp;
+                    assert validityPredicates[vpn] == s_w_honest_node_states_updated.honest_nodes_states[vpn].block_consensus_engine_state.active_consensus_instances_on_beacon_blocks[cid].validityPredicate;
+                    assert vpn in s.honest_nodes_states.Keys;
+                    assert cid in s_w_honest_node_states_updated.honest_nodes_states[vpn].block_consensus_engine_state.active_consensus_instances_on_beacon_blocks.Keys;
+
+                    lem_inv_sent_validity_predicate_is_based_on_rcvd_proposer_duty_and_slashing_db_and_randao_reveal_get_s_w_honest_node_states_updated_2(s, node, nodeEvent, vpn, s_w_honest_node_states_updated);
+
+                    assert s_w_honest_node_states_updated.honest_nodes_states[vpn].block_consensus_engine_state == s.honest_nodes_states[vpn].block_consensus_engine_state;
+                    assert inv_sent_validity_predicate_is_based_on_rcvd_proposer_duty_and_slashing_db_and_randao_reveal_for_dvc_single_dvc(s, vpn, cid);
+
+                    proposer_duty, block_slashing_db, randao_reveal :| inv_sent_validity_predicate_is_based_on_rcvd_proposer_duty_and_slashing_db_and_randao_reveal_body(cid, proposer_duty, block_slashing_db, randao_reveal, vp);
                 }
 
-            case AdversaryTakingStep(node, new_attestation_shares_sent, messagesReceivedByTheNode) =>
-                assert inv_rcvd_att_duty_is_from_dv_seq_for_rcvd_att_duty(dv');        
-                
-        }   
-    }  
+                assert inv_sent_validity_predicate_is_based_on_rcvd_proposer_duty_and_slashing_db_and_randao_reveal_body(cid, proposer_duty, block_slashing_db, randao_reveal, vp);
+        }
 
+    }
+
+    lemma lem_inv_sent_validity_predicate_is_based_on_rcvd_proposer_duty_and_slashing_db_and_randao_reveal_dv_next(
+        s: DVState,
+        event: DV_Block_Proposer_Spec.Event,
+        s': DVState
+    )
+    requires NextEventPreCond(s, event)
+    requires NextEvent(s, event, s')
+    requires inv_sent_validity_predicate_is_based_on_rcvd_proposer_duty_and_slashing_db_and_randao_reveal(s)
+    requires inv_quorum_constraints(s)
+    requires inv_unchanged_paras_of_consensus_instances(s)
+    requires inv_only_dv_construct_complete_signed_block(s)
+    requires inv_sent_validity_predicate_is_based_on_rcvd_proposer_duty_and_slashing_db_and_randao_reveal_for_dv(s)
+    ensures inv_sent_validity_predicate_is_based_on_rcvd_proposer_duty_and_slashing_db_and_randao_reveal(s')
+    {
+        match event
+        {
+            case HonestNodeTakingStep(node, nodeEvent, nodeOutputs) =>
+                forall hn, cid: Slot, vp |
+                    && hn in s'.consensus_instances_on_beacon_block[cid].honest_nodes_validity_functions.Keys
+                    && vp in s'.consensus_instances_on_beacon_block[cid].honest_nodes_validity_functions[hn]
+                ensures exists proposer_duty, block_slashing_db, randao_reveal :: inv_sent_validity_predicate_is_based_on_rcvd_proposer_duty_and_slashing_db_and_randao_reveal_body(cid, proposer_duty, block_slashing_db, randao_reveal, vp)
+                {
+                    var proposer_duty: ProposerDuty, block_slashing_db, randao_reveal := lem_inv_sent_validity_predicate_is_based_on_rcvd_proposer_duty_and_slashing_db_and_randao_reveal_helper(s, event, s', cid, hn, vp);
+                }
+                assert inv_sent_validity_predicate_is_based_on_rcvd_proposer_duty_and_slashing_db_and_randao_reveal(s');
+
+            case AdversaryTakingStep(node, new_randao_shares_sent, new_sent_block_shares, randaoShareReceivedByTheNode, blockShareReceivedByTheNode) =>
+                assert inv_sent_validity_predicate_is_based_on_rcvd_proposer_duty_and_slashing_db_and_randao_reveal(s');
+        }
+    }
+    
     
 
-    lemma lem_inv_none_latest_att_duty_and_empty_set_of_rcvd_att_duties_dv_next(
-        dv: DVState,
-        event: DV.Event,
-        dv': DVState
-    )    
-    requires NextEventPreCond(dv, event)
-    requires NextEvent(dv, event, dv')  
-    requires inv_none_latest_att_duty_and_empty_set_of_rcvd_att_duties(dv)
-    ensures inv_none_latest_att_duty_and_empty_set_of_rcvd_att_duties(dv')
-    {  
+    lemma lem_inv_block_of_in_transit_block_share_is_decided_value_when_no_new_block_share_is_added_helper<M>(
+        allMessagesSent': set<M>,
+        allMessagesSent: set<M>,
+        messagesToBeSent: set<MessaageWithRecipient<M>>
+    )
+    requires allMessagesSent' == allMessagesSent +
+                                getMessagesFromMessagesWithRecipient(messagesToBeSent);
+    requires messagesToBeSent == {}
+    ensures allMessagesSent' == allMessagesSent
+    { }
 
-        match event 
+    lemma lem_inv_block_of_in_transit_block_share_is_decided_value_when_no_new_block_share_is_added(
+        s: DVState,
+        event: DV_Block_Proposer_Spec.Event,
+        s': DVState
+    )
+    requires NextEventPreCond(s, event)
+    requires NextEvent(s, event, s')
+    requires inv_block_of_in_transit_block_share_is_decided_value(s)
+    requires inv_quorum_constraints(s)
+    requires inv_same_node_status_in_dv_and_ci(s)
+    requires s'.block_share_network.allMessagesSent ==
+                    s.block_share_network.allMessagesSent + getMessagesFromMessagesWithRecipient({});
+    ensures  inv_block_of_in_transit_block_share_is_decided_value(s');
+    {
+        forall cid | cid in s.consensus_instances_on_beacon_block.Keys
+        ensures && var s_consensus := s.consensus_instances_on_beacon_block[cid];
+                && var s'_consensus := s'.consensus_instances_on_beacon_block[cid];
+                && s_consensus.decided_value.isPresent() ==>
+                        ( && s'_consensus.decided_value.isPresent()
+                          && s_consensus.decided_value.safe_get() == s'_consensus.decided_value.safe_get()
+                        )
+            ;
         {
-            case HonestNodeTakingStep(node, nodeEvent, nodeOutputs) =>
-                var dvc := dv.honest_nodes_states[node];
-                var dvc' := dv'.honest_nodes_states[node];
-                match nodeEvent
-                {
-                    case ServeAttestationDuty(attestation_duty) =>    
-                        lem_inv_none_latest_att_duty_and_empty_set_of_rcvd_att_duties_body_f_serve_attestation_duty(
-                            dvc,
-                            attestation_duty,
-                            dvc'
-                        );
-                        assert inv_none_latest_att_duty_and_empty_set_of_rcvd_att_duties(dv'); 
-                        
+            var s_consensus := s.consensus_instances_on_beacon_block[cid];
+            var s'_consensus := s'.consensus_instances_on_beacon_block[cid];
 
-                    case AttConsensusDecided(id, decided_attestation_data) => 
-                        assert inv_none_latest_att_duty_and_empty_set_of_rcvd_att_duties(dv');         
+            assert isConditionForSafetyTrue(s_consensus);
+            assert s_consensus.decided_value.isPresent() ==>
+                && s'_consensus.decided_value.isPresent()
+                && s_consensus.decided_value.safe_get() == s'_consensus.decided_value.safe_get()
+            ;
+        }
 
-                    case ReceivedAttestationShare(attestation_share) =>   
-                        assert inv_none_latest_att_duty_and_empty_set_of_rcvd_att_duties(dv');              
-   
-                    case ImportedNewBlock(block) => 
-                        assert inv_none_latest_att_duty_and_empty_set_of_rcvd_att_duties(dv');     
-                                          
-                    case ResendAttestationShares =>  
-                        assert inv_none_latest_att_duty_and_empty_set_of_rcvd_att_duties(dv');     
+        assert forall cid | cid in s.consensus_instances_on_beacon_block.Keys ::
+                    && var s_consensus := s.consensus_instances_on_beacon_block[cid];
+                    && var s'_consensus := s'.consensus_instances_on_beacon_block[cid];
+                    && s_consensus.decided_value.isPresent() ==>
+                            ( && s'_consensus.decided_value.isPresent()
+                            && s_consensus.decided_value.safe_get() == s'_consensus.decided_value.safe_get()
+                            )
+        ;
 
-                    case NoEvent => 
-                        assert dvc == dvc'; 
-                        assert dvc.all_rcvd_duties == dvc'.all_rcvd_duties;  
-                        assert inv_none_latest_att_duty_and_empty_set_of_rcvd_att_duties(dv'); 
-                }
+        var emptySet: set<MessaageWithRecipient<SignedBeaconBlock>> := {};
+        calc {
+            s'.block_share_network.allMessagesSent;
+            ==
+            s.block_share_network.allMessagesSent + getMessagesFromMessagesWithRecipient(emptySet);
+            ==
+            {lem_getMessagesFromEmptySetOfMessagesWithRecipient_is_empty_set(emptySet);}
+            s.block_share_network.allMessagesSent;
+        }
 
-            case AdversaryTakingStep(node, new_attestation_shares_sent, messagesReceivedByTheNode) =>
-                assert inv_none_latest_att_duty_and_empty_set_of_rcvd_att_duties(dv');        
-                
-        }   
+        assert s'.block_share_network.allMessagesSent == s.block_share_network.allMessagesSent;
+
+        forall hn, block_share |
+                && hn in s'.honest_nodes_states.Keys
+                && block_share in s'.block_share_network.allMessagesSent
+                && var block_signing_root := compute_block_signing_root(block_share.block);
+                && verify_bls_signature(block_signing_root, block_share.signature, hn)
+        ensures inv_block_of_in_transit_block_share_is_decided_value_body(s', block_share);
+        {
+            assert block_share in s.block_share_network.allMessagesSent;
+            assert inv_block_of_in_transit_block_share_is_decided_value_body(s, block_share);
+            assert inv_block_of_in_transit_block_share_is_decided_value_body(s', block_share);
+        }
+
+        assert inv_block_of_in_transit_block_share_is_decided_value(s');
     }
 
-    lemma lem_inv_no_rcvd_att_duty_is_higher_than_latest_att_duty_dv_next(
-        dv: DVState,
-        event: DV.Event,
-        dv': DVState
-    )    
-    requires NextEventPreCond(dv, event)
-    requires NextEvent(dv, event, dv')  
-    requires inv_no_rcvd_att_duty_is_higher_than_latest_att_duty(dv)
-    requires inv_none_latest_att_duty_and_empty_set_of_rcvd_att_duties(dv)
-    ensures inv_no_rcvd_att_duty_is_higher_than_latest_att_duty(dv')
-    {  
+     lemma lem_consensus_decision_is_unchanged<D(!new, 0)>(
+        s: BlockConsensusInstance,
+        honest_nodes_validity_predicates: map<BLSPubkey, D -> bool>,
+        s': BlockConsensusInstance,
+        output: Optional<OutCommand>
+    )
+    requires Block_Consensus_Spec.Next(s, honest_nodes_validity_predicates, s', output)
+    requires isConditionForSafetyTrue(s)
+    requires s.decided_value.isPresent()
+    ensures s'.decided_value.isPresent()
+    ensures s.decided_value.safe_get() == s'.decided_value.safe_get()
+    { }
 
-        match event 
-        {
-            case HonestNodeTakingStep(node, nodeEvent, nodeOutputs) =>
-                var dvc := dv.honest_nodes_states[node];
-                var dvc' := dv'.honest_nodes_states[node];
-                match nodeEvent
-                {
-                    case ServeAttestationDuty(attestation_duty) =>    
-                        lem_inv_no_rcvd_att_duty_is_higher_than_latest_att_duty_body_f_serve_attestation_duty(
-                            dvc,
-                            attestation_duty,
-                            dvc'
-                        );
-                        assert inv_none_latest_att_duty_and_empty_set_of_rcvd_att_duties(dv'); 
-                        
-
-                    case AttConsensusDecided(id, decided_attestation_data) => 
-                        assert inv_no_rcvd_att_duty_is_higher_than_latest_att_duty(dv');         
-
-                    case ReceivedAttestationShare(attestation_share) =>   
-                        assert inv_no_rcvd_att_duty_is_higher_than_latest_att_duty(dv');              
-   
-                    case ImportedNewBlock(block) => 
-                        assert inv_no_rcvd_att_duty_is_higher_than_latest_att_duty(dv');     
-                                          
-                    case ResendAttestationShares =>  
-                        assert inv_no_rcvd_att_duty_is_higher_than_latest_att_duty(dv');     
-
-                    case NoEvent => 
-                        assert dvc == dvc'; 
-                        assert dvc.all_rcvd_duties == dvc'.all_rcvd_duties;  
-                        assert inv_no_rcvd_att_duty_is_higher_than_latest_att_duty(dv'); 
-                }
-
-            case AdversaryTakingStep(node, new_attestation_shares_sent, messagesReceivedByTheNode) =>
-                assert inv_no_rcvd_att_duty_is_higher_than_latest_att_duty(dv');        
-                
-        }   
+    predicate is_correct_block_share(
+        s: DVState,
+        hn: BLSPubkey,
+        block_share: SignedBeaconBlock
+    )
+    {
+        && hn in s.honest_nodes_states.Keys 
+        && block_share in s.block_share_network.allMessagesSent
+        && var block_signing_root := compute_block_signing_root(block_share.block);
+        && verify_bls_signature(block_signing_root, block_share.signature, hn)   
     }
 
-
-    lemma lem_inv_unique_rcvd_att_duty_per_slot_dv_next(
-        dv: DVState,
-        event: DV.Event,
-        dv': DVState
-    )    
-    requires NextEventPreCond(dv, event)
-    requires NextEvent(dv, event, dv')  
-    requires inv_unique_rcvd_att_duty_per_slot(dv)
-    requires inv_no_rcvd_att_duty_is_higher_than_latest_att_duty(dv)
-    requires inv_none_latest_att_duty_and_empty_set_of_rcvd_att_duties(dv)
-    ensures inv_unique_rcvd_att_duty_per_slot(dv')
-    {  
-
-        match event 
+    lemma lem_inv_block_of_in_transit_block_share_is_decided_value_BlockConsensusDecided_block_of_inputs_is_decision_of_consensus_instance(
+        s: DVState,
+        event: DV_Block_Proposer_Spec.Event,
+        s': DVState,
+        hn: BLSPubkey,
+        block_share: SignedBeaconBlock
+    )
+    requires NextEventPreCond(s, event)
+    requires NextEvent(s, event, s')
+    requires event.HonestNodeTakingStep?
+    requires event.event.BlockConsensusDecided?
+    requires inv_quorum_constraints(s)
+    requires inv_same_node_status_in_dv_and_ci(s)
+    requires is_correct_block_share(s, hn, block_share)
+    requires inv_block_of_in_transit_block_share_is_decided_value(s)
+    requires block_share in s.block_share_network.allMessagesSent
+    ensures && s'.consensus_instances_on_beacon_block[block_share.block.slot].decided_value.isPresent()
+            && s'.consensus_instances_on_beacon_block[block_share.block.slot].decided_value.safe_get() == block_share.block
+    {
+        match event
         {
             case HonestNodeTakingStep(node, nodeEvent, nodeOutputs) =>
-                var dvc := dv.honest_nodes_states[node];
-                var dvc' := dv'.honest_nodes_states[node];
+                var s_node := s.honest_nodes_states[node];
+                var s'_node := s'.honest_nodes_states[node];
                 match nodeEvent
                 {
-                    case ServeAttestationDuty(attestation_duty) =>    
-                        if !dvc.latest_attestation_duty.isPresent()                            
+                    case BlockConsensusDecided(id: Slot, decided_beacon_block) =>
+                        assert inv_block_of_in_transit_block_share_is_decided_value_body(s, block_share);
+                        assert s.consensus_instances_on_beacon_block[block_share.block.slot].decided_value.isPresent();
+                        assert s.consensus_instances_on_beacon_block[block_share.block.slot].decided_value.safe_get() == block_share.block;
+
+                        var s_w_honest_node_states_updated := f_inv_sent_validity_predicate_is_based_on_rcvd_proposer_duty_and_slashing_db_and_randao_reveal_get_s_w_honest_node_states_updated(s, node, nodeEvent);
+                        var cid := block_share.block.slot;
+
+                        assert s_w_honest_node_states_updated.consensus_instances_on_beacon_block == s.consensus_instances_on_beacon_block;
+
+                        var output :=
+                            if nodeEvent.BlockConsensusDecided? && nodeEvent.id == cid 
+                            then
+                                Some(Decided(node, nodeEvent.decided_beacon_block))
+                            else
+                                None
+                            ;
+
+                        var validityPredicates :=
+                            map n |
+                                    && n in s_w_honest_node_states_updated.honest_nodes_states.Keys
+                                    && cid in s_w_honest_node_states_updated.honest_nodes_states[n].block_consensus_engine_state.active_consensus_instances_on_beacon_blocks.Keys
+                                ::
+                                    s_w_honest_node_states_updated.honest_nodes_states[n].block_consensus_engine_state.active_consensus_instances_on_beacon_blocks[cid].validityPredicate
+                            ;
+
+                        var s_consensus := s_w_honest_node_states_updated.consensus_instances_on_beacon_block[cid];
+                        var s'_consensus := s'.consensus_instances_on_beacon_block[cid];
+
+                        assert  Block_Consensus_Spec.Next(
+                                    s_consensus,
+                                    validityPredicates,
+                                    s'_consensus,
+                                    output
+                                );
+
+                        lem_consensus_decision_is_unchanged(
+                            s_consensus,
+                            validityPredicates,
+                            s'_consensus,
+                            output
+                        );
+                }
+        }
+    }
+
+    lemma lem_inv_block_of_in_transit_block_share_is_decided_value_BlockConsensusDecided_with_decided_data_for_current_slot(
+        s: DVState,
+        event: DV_Block_Proposer_Spec.Event,
+        s': DVState,
+        node: BLSPubkey,
+        nodeEvent: Block_Types.Event,
+        nodeOutputs: Outputs,
+        id: Slot,
+        decided_beacon_block: BeaconBlock
+    )
+    requires NextEventPreCond(s, event)
+    requires NextEvent(s, event, s')
+    requires event.HonestNodeTakingStep?
+    requires event == HonestNodeTakingStep(node, nodeEvent, nodeOutputs)
+    requires nodeEvent.BlockConsensusDecided?
+    requires nodeEvent == BlockConsensusDecided(id, decided_beacon_block)
+    requires inv_block_of_in_transit_block_share_is_decided_value(s)
+    requires inv_decided_value_of_consensus_instance_of_slot_k_is_for_slot_k(s)
+    requires inv_block_shares_to_broadcast_is_a_subset_of_all_sent_messages(s)
+    requires inv_same_node_status_in_dv_and_ci(s)
+    requires inv_decided_value_of_consensus_instance_is_decided_by_quorum(s)
+    requires inv_sent_validity_predicate_is_based_on_rcvd_proposer_duty_and_slashing_db_and_randao_reveal(s)
+    requires inv_sent_validity_predicate_is_based_on_rcvd_proposer_duty_and_slashing_db_and_randao_reveal_for_dv(s)
+    requires && var process := s.honest_nodes_states[node];
+             && process.current_proposer_duty.isPresent()
+             && process.current_proposer_duty.safe_get().slot == decided_beacon_block.slot
+             && id == decided_beacon_block.slot
+    requires inv_quorum_constraints(s)
+    requires inv_unchanged_paras_of_consensus_instances(s) 
+    requires inv_only_dv_construct_complete_signing_functions(s)
+    ensures inv_block_of_in_transit_block_share_is_decided_value(s')
+    {   
+        assert inv_only_dv_construct_complete_signed_block(s);
+
+        var process := s.honest_nodes_states[node];
+        var process' := s'.honest_nodes_states[node];
+
+        var slot := decided_beacon_block.slot;
+        var block_signing_root := compute_block_signing_root(decided_beacon_block);
+        var fork_version := bn_get_fork_version(slot);
+        var block_signature := rs_sign_block(decided_beacon_block, fork_version, block_signing_root, process.rs);
+        var block_share := SignedBeaconBlock(decided_beacon_block, block_signature);
+        
+        var messagesToBeSent := f_block_consensus_decided(process, id, decided_beacon_block).outputs.sent_block_shares;
+
+        assert  messagesToBeSent ==  multicast(block_share, process.peers);
+        assert  s'.block_share_network.allMessagesSent ==
+                s.block_share_network.allMessagesSent + getMessagesFromMessagesWithRecipient(messagesToBeSent);
+        assert forall m | m in messagesToBeSent :: m.message == block_share;
+
+        lemmaOnGetMessagesFromMessagesWithRecipientWhenAllMessagesAreTheSame(messagesToBeSent, block_share);
+        assert getMessagesFromMessagesWithRecipient(messagesToBeSent) == {block_share};
+        assert  s'.block_share_network.allMessagesSent ==
+                s.block_share_network.allMessagesSent + { block_share };
+
+        forall hn, block_share |
+                && hn in s'.honest_nodes_states.Keys
+                && block_share in s'.block_share_network.allMessagesSent
+                && var block_signing_root := compute_block_signing_root(block_share.block);
+                && verify_bls_signature(block_signing_root, block_share.signature, hn)
+        ensures s'.consensus_instances_on_beacon_block[block_share.block.slot].decided_value.isPresent();
+        ensures s'.consensus_instances_on_beacon_block[block_share.block.slot].decided_value.safe_get() == block_share.block;
+        {
+            if block_share in s.block_share_network.allMessagesSent
+            {
+                lem_inv_block_of_in_transit_block_share_is_decided_value_BlockConsensusDecided_block_of_inputs_is_decision_of_consensus_instance(s, event, s', hn, block_share);
+            }
+            else
+            {
+                assert block_share == block_share;
+                lemmaImaptotalElementInDomainIsInKeys(s.consensus_instances_on_beacon_block, id);
+                assert id in s.consensus_instances_on_beacon_block.Keys ;
+                 
+                lem_inv_block_of_in_transit_block_share_is_decided_value_BlockConsensusDecided_block_in_inputs_is_decided_value(s, event, s');
+                assert s'.consensus_instances_on_beacon_block[id].decided_value.safe_get() == decided_beacon_block;
+                assert s'.consensus_instances_on_beacon_block[id].decided_value.safe_get() == block_share.block;
+
+                lem_inv_decided_value_of_consensus_instance_of_slot_k_is_for_slot_k_dv_next(s, event, s');
+            }
+        }
+
+        assert inv_block_of_in_transit_block_share_is_decided_value(s');
+    }
+
+    lemma lem_inv_block_of_in_transit_block_share_is_decided_value_dv_next_ServeProposerDuty(
+        s: DVState,
+        event: DV_Block_Proposer_Spec.Event,
+        s': DVState
+    )
+    requires NextEventPreCond(s, event)
+    requires NextEvent(s, event, s')
+    requires event.HonestNodeTakingStep?
+    requires event.event.ServeProposerDuty?
+    requires inv_quorum_constraints(s)
+    requires inv_same_node_status_in_dv_and_ci(s)
+    requires inv_block_of_in_transit_block_share_is_decided_value(s)
+    ensures inv_block_of_in_transit_block_share_is_decided_value(s')
+    {
+        match event
+        {
+            case HonestNodeTakingStep(node, nodeEvent, nodeOutputs) =>
+                var s_node := s.honest_nodes_states[node];
+                var s'_node := s'.honest_nodes_states[node];
+                match nodeEvent
+                {
+                    case ServeProposerDuty(proposer_duty) =>
+                        var sentBlockShares := f_serve_proposer_duty(s_node, proposer_duty).outputs.sent_block_shares;
+
+                        lem_f_serve_proposer_duty_unchanged_vars(s_node, proposer_duty, s'_node);
+                        assert  sentBlockShares == {};
+                        assert  s'.block_share_network.allMessagesSent ==
+                                s.block_share_network.allMessagesSent + getMessagesFromMessagesWithRecipient(sentBlockShares);
+                        lem_inv_block_of_in_transit_block_share_is_decided_value_when_no_new_block_share_is_added_helper(s'.block_share_network.allMessagesSent, s.block_share_network.allMessagesSent, sentBlockShares);
+                        assert s'.block_share_network.allMessagesSent == s.block_share_network.allMessagesSent;
+                        lem_inv_block_of_in_transit_block_share_is_decided_value_when_no_new_block_share_is_added(s, event, s');
+                }
+        }
+    }
+
+    lemma lem_inv_block_of_in_transit_block_share_is_decided_value_dv_next_ReceiveRandaoShare(
+        s: DVState,
+        event: DV_Block_Proposer_Spec.Event,
+        s': DVState
+    )
+    requires NextEventPreCond(s, event)
+    requires NextEvent(s, event, s')
+    requires event.HonestNodeTakingStep?
+    requires event.event.ReceiveRandaoShare?
+    requires inv_quorum_constraints(s)
+    requires inv_same_node_status_in_dv_and_ci(s)
+    requires inv_block_of_in_transit_block_share_is_decided_value(s)
+    ensures inv_block_of_in_transit_block_share_is_decided_value(s')
+    {
+        match event
+        {
+            case HonestNodeTakingStep(node, nodeEvent, nodeOutputs) =>
+                var s_node := s.honest_nodes_states[node];
+                var s'_node := s'.honest_nodes_states[node];
+                match nodeEvent
+                {
+                    case ReceiveRandaoShare(randao_share) =>
+                        var sentBlockShares := f_listen_for_randao_shares(s_node, randao_share).outputs.sent_block_shares;
+
+                        lem_f_listen_for_randao_shares_unchanged_vars(s_node, randao_share, s'_node);
+                        assert  sentBlockShares == {};
+                        assert  s'.block_share_network.allMessagesSent ==
+                                s.block_share_network.allMessagesSent + getMessagesFromMessagesWithRecipient(sentBlockShares);
+                        lem_inv_block_of_in_transit_block_share_is_decided_value_when_no_new_block_share_is_added_helper(s'.block_share_network.allMessagesSent, s.block_share_network.allMessagesSent, sentBlockShares);
+                        assert s'.block_share_network.allMessagesSent == s.block_share_network.allMessagesSent;
+                        lem_inv_block_of_in_transit_block_share_is_decided_value_when_no_new_block_share_is_added(s, event, s');
+                }
+        }
+    }
+
+    lemma lem_inv_block_of_in_transit_block_share_is_decided_value_BlockConsensusDecided_block_in_inputs_is_decided_value(
+        s: DVState,
+        event: DV_Block_Proposer_Spec.Event,
+        s': DVState
+    )
+    requires NextEventPreCond(s, event)
+    requires NextEvent(s, event, s')
+    requires event.HonestNodeTakingStep?
+    requires event.event.BlockConsensusDecided?
+    requires inv_quorum_constraints(s)
+    requires inv_unchanged_paras_of_consensus_instances(s)
+    ensures s'.consensus_instances_on_beacon_block[event.event.id].decided_value.safe_get() == event.event.decided_beacon_block;
+    {
+        match event
+        {
+            case HonestNodeTakingStep(node, nodeEvent, nodeOutputs) =>
+                var s_node := s.honest_nodes_states[node];
+                var s'_node := s'.honest_nodes_states[node];
+                match nodeEvent
+                {
+                    case BlockConsensusDecided(id: Slot, decided_beacon_block) =>
+                        var s_w_honest_node_states_updated := f_inv_sent_validity_predicate_is_based_on_rcvd_proposer_duty_and_slashing_db_and_randao_reveal_get_s_w_honest_node_states_updated(s, node, nodeEvent);
+                        var cid := id;
+
+                        assert s_w_honest_node_states_updated.consensus_instances_on_beacon_block == s.consensus_instances_on_beacon_block;
+
+                        var output := Some(Decided(node, nodeEvent.decided_beacon_block));
+
+                        var validityPredicates :=
+                                map n |
+                                        && n in s_w_honest_node_states_updated.honest_nodes_states.Keys
+                                        && cid in s_w_honest_node_states_updated.honest_nodes_states[n].block_consensus_engine_state.active_consensus_instances_on_beacon_blocks.Keys
+                                    ::
+                                        s_w_honest_node_states_updated.honest_nodes_states[n].block_consensus_engine_state.active_consensus_instances_on_beacon_blocks[cid].validityPredicate
+                                ;
+
+                        var s_consensus := s_w_honest_node_states_updated.consensus_instances_on_beacon_block[cid];
+                        var s'_consensus := s'.consensus_instances_on_beacon_block[cid];
+
+                        assert Block_Consensus_Spec.Next(
+                                    s_consensus,
+                                    validityPredicates,
+                                    s'_consensus,
+                                    output
+                                );
+
+                        assert s'.consensus_instances_on_beacon_block[id].decided_value.isPresent();
+                        assert isConditionForSafetyTrue(s'_consensus);
+                        assert s'_consensus.decided_value.safe_get() == decided_beacon_block;
+                        assert s'.consensus_instances_on_beacon_block[id].decided_value.safe_get() == decided_beacon_block;
+                }
+        }
+    }
+
+    lemma lem_inv_block_of_in_transit_block_share_is_decided_value_BlockConsensusDecided(
+        s: DVState,
+        event: DV_Block_Proposer_Spec.Event,
+        s': DVState
+    )
+    requires NextEventPreCond(s, event)
+    requires NextEvent(s, event, s')
+    requires event.HonestNodeTakingStep?
+    requires event.event.BlockConsensusDecided?
+    requires inv_block_of_in_transit_block_share_is_decided_value(s)
+    requires inv_decided_value_of_consensus_instance_of_slot_k_is_for_slot_k(s)
+    requires inv_block_shares_to_broadcast_is_a_subset_of_all_sent_messages(s)
+    requires inv_quorum_constraints(s)
+    requires inv_unchanged_paras_of_consensus_instances(s)
+    requires inv_same_node_status_in_dv_and_ci(s)
+    requires inv_only_dv_construct_complete_signing_functions(s)
+    requires inv_decided_value_of_consensus_instance_is_decided_by_quorum(s)
+    requires inv_sent_validity_predicate_is_based_on_rcvd_proposer_duty_and_slashing_db_and_randao_reveal(s)
+    requires inv_sent_validity_predicate_is_based_on_rcvd_proposer_duty_and_slashing_db_and_randao_reveal_for_dv(s)
+    ensures inv_block_of_in_transit_block_share_is_decided_value(s')
+    {
+        match event
+        {
+            case HonestNodeTakingStep(node, nodeEvent, nodeOutputs) =>
+                var process := s.honest_nodes_states[node];
+                var process' := s'.honest_nodes_states[node];
+                match nodeEvent
+                {
+                    case BlockConsensusDecided(id: Slot, decided_beacon_block) =>
+                        if  && process.current_proposer_duty.isPresent()
+                            && process.current_proposer_duty.safe_get().slot == decided_beacon_block.slot
+                            && id == decided_beacon_block.slot
                         {
-                            lem_inv_none_latest_att_duty_and_empty_set_of_rcvd_att_duties_dv_next(dv, event, dv');
-                            assert dvc'.all_rcvd_duties == {attestation_duty};
-                            assert inv_unique_rcvd_att_duty_per_slot(dv');
+                            lem_inv_block_of_in_transit_block_share_is_decided_value_BlockConsensusDecided_with_decided_data_for_current_slot(
+                                s,
+                                event,
+                                s',
+                                node,
+                                nodeEvent,
+                                nodeOutputs,
+                                id,
+                                decided_beacon_block
+                            );
                         }
                         else
                         {
-                            if dvc.latest_attestation_duty.safe_get().slot < attestation_duty.slot
-                            {
-                                assert attestation_duty !in dvc.all_rcvd_duties;
-                                assert inv_unique_rcvd_att_duty_per_slot(dv');     
-                            }   
-                            else
-                            {
-                                assert inv_unique_rcvd_att_duty_per_slot(dv');     
-                            }                            
+                            var sentBlockShares := f_block_consensus_decided(process, id, decided_beacon_block).outputs.sent_block_shares;
+
+                            assert  sentBlockShares == {};
+                            assert  s'.block_share_network.allMessagesSent ==
+                                    s.block_share_network.allMessagesSent + getMessagesFromMessagesWithRecipient(sentBlockShares);
+                            lem_inv_block_of_in_transit_block_share_is_decided_value_when_no_new_block_share_is_added_helper(s'.block_share_network.allMessagesSent, s.block_share_network.allMessagesSent, sentBlockShares);
+                            assert s'.block_share_network.allMessagesSent == s.block_share_network.allMessagesSent;
+                            lem_inv_block_of_in_transit_block_share_is_decided_value_when_no_new_block_share_is_added(s, event, s');
                         }
+                }
+        }
+    }
+
+    lemma lem_inv_block_of_in_transit_block_share_is_decided_value_dv_next_ReceiveSignedBeaconBlock(
+        s: DVState,
+        event: DV_Block_Proposer_Spec.Event,
+        s': DVState
+    )
+    requires NextEventPreCond(s, event)
+    requires NextEvent(s, event, s')
+    requires event.HonestNodeTakingStep?
+    requires event.event.ReceiveSignedBeaconBlock?
+    requires inv_quorum_constraints(s)
+    requires inv_same_node_status_in_dv_and_ci(s)
+    requires inv_block_of_in_transit_block_share_is_decided_value(s)
+    ensures inv_block_of_in_transit_block_share_is_decided_value(s')
+    {
+        match event
+        {
+            case HonestNodeTakingStep(node, nodeEvent, nodeOutputs) =>
+                var s_node := s.honest_nodes_states[node];
+                var s'_node := s'.honest_nodes_states[node];
+                match nodeEvent
+                {
+                    case ReceiveSignedBeaconBlock(block_share) =>
+                        var sentBlockShares := f_listen_for_block_signature_shares(s_node, block_share).outputs.sent_block_shares;
+
+                        lem_f_listen_for_block_signature_shares_unchanged_vars(s_node, block_share, s'_node);
+                        assert  sentBlockShares == {};
+                        assert  s'.block_share_network.allMessagesSent ==
+                                s.block_share_network.allMessagesSent + getMessagesFromMessagesWithRecipient(sentBlockShares);
+                        lem_inv_block_of_in_transit_block_share_is_decided_value_when_no_new_block_share_is_added_helper(s'.block_share_network.allMessagesSent, s.block_share_network.allMessagesSent, sentBlockShares);
+                        assert s'.block_share_network.allMessagesSent == s.block_share_network.allMessagesSent;
+                        lem_inv_block_of_in_transit_block_share_is_decided_value_when_no_new_block_share_is_added(s, event, s');
+                }
+        }
+    }
+
+    lemma lem_inv_block_of_in_transit_block_share_is_decided_value_dv_next_ImportedNewBlock(
+        s: DVState,
+        event: DV_Block_Proposer_Spec.Event,
+        s': DVState
+    )
+    requires NextEventPreCond(s, event)
+    requires NextEvent(s, event, s')
+    requires event.HonestNodeTakingStep?
+    requires event.event.ImportedNewBlock?
+    requires inv_quorum_constraints(s)
+    requires inv_same_node_status_in_dv_and_ci(s)
+    requires inv_block_of_in_transit_block_share_is_decided_value(s)
+    ensures inv_block_of_in_transit_block_share_is_decided_value(s')
+    {
+        match event
+        {
+            case HonestNodeTakingStep(node, nodeEvent, nodeOutputs) =>
+                var s_node := s.honest_nodes_states[node];
+                var s'_node := s'.honest_nodes_states[node];
+                match nodeEvent
+                {
+                    case ImportedNewBlock(block) =>
+                        var s_node := f_add_block_to_bn(s_node, nodeEvent.block);                        
+                        var messagesToBeSent := f_listen_for_new_imported_blocks(s_node, block).outputs.sent_block_shares;
+                        assert f_listen_for_new_imported_blocks.requires(s_node, block);
+                        assert s'_node == f_listen_for_new_imported_blocks(s_node, block).state;                        
+
+                        lem_f_listen_for_new_imported_blocks_unchanged_dvc_vars(s_node, block, s'_node);
+                        assert messagesToBeSent == {};
+                        assert  s'.block_share_network.allMessagesSent ==
+                                s.block_share_network.allMessagesSent + getMessagesFromMessagesWithRecipient(messagesToBeSent);                        
                         
+                        lem_inv_block_of_in_transit_block_share_is_decided_value_when_no_new_block_share_is_added_helper(s'.block_share_network.allMessagesSent, s.block_share_network.allMessagesSent, messagesToBeSent);
+                        assert s'.block_share_network.allMessagesSent == s.block_share_network.allMessagesSent;
+                        
+                        lem_inv_block_of_in_transit_block_share_is_decided_value_when_no_new_block_share_is_added(s, event, s');
+                }
+        }
+    }
 
-                    case AttConsensusDecided(id, decided_attestation_data) => 
-                        assert inv_unique_rcvd_att_duty_per_slot(dv');         
+    lemma lem_inv_block_of_in_transit_block_share_is_decided_value_dv_next_ResendBlockShare(
+        s: DVState,
+        event: DV_Block_Proposer_Spec.Event,
+        s': DVState
+    )
+    requires NextEventPreCond(s, event)
+    requires NextEvent(s, event, s')
+    requires event.HonestNodeTakingStep?
+    requires event.event.ResendBlockShare?
+    requires inv_quorum_constraints(s)
+    requires inv_same_node_status_in_dv_and_ci(s)
+    requires inv_block_of_in_transit_block_share_is_decided_value(s)
+    requires inv_block_shares_to_broadcast_is_a_subset_of_all_sent_messages(s)
+    ensures inv_block_of_in_transit_block_share_is_decided_value(s')
+    {
+        match event
+        {
+            case HonestNodeTakingStep(node, nodeEvent, nodeOutputs) =>
+                var s_node := s.honest_nodes_states[node];
+                var s'_node := s'.honest_nodes_states[node];
+                match nodeEvent
+                {
+                    case ResendBlockShare =>
+                        var messagesToBeSent := f_resend_block_share(s_node).outputs.sent_block_shares;
 
-                    case ReceivedAttestationShare(attestation_share) =>   
-                        assert inv_unique_rcvd_att_duty_per_slot(dv');              
+                            assert s'.block_share_network.allMessagesSent ==
+                                        s.block_share_network.allMessagesSent + getMessagesFromMessagesWithRecipient(messagesToBeSent);
+
+                            forall m | m in getMessagesFromMessagesWithRecipient(messagesToBeSent)
+                            ensures m in s.block_share_network.allMessagesSent
+                            {
+                                assert m in s_node.block_shares_to_broadcast.Values;
+                                assert m in s.block_share_network.allMessagesSent;
+                            }
+
+                            assert s'.block_share_network.allMessagesSent == s.block_share_network.allMessagesSent;
+                            lem_inv_block_of_in_transit_block_share_is_decided_value_when_no_new_block_share_is_added(s, event, s');
+                }
+        }
+    }
+
+    lemma lem_inv_block_of_in_transit_block_share_is_decided_value_proposer_adversary(
+        s: DVState,
+        event: DV_Block_Proposer_Spec.Event,
+        s': DVState
+    )
+    requires NextEventPreCond(s, event)
+    requires NextEvent(s, event, s')
+    requires event.AdversaryTakingStep?
+    requires inv_block_of_in_transit_block_share_is_decided_value(s)
+    requires inv_quorum_constraints(s)
+    requires inv_same_node_status_in_dv_and_ci(s)
+    requires inv_only_dv_construct_complete_signed_block(s)
+    ensures inv_block_of_in_transit_block_share_is_decided_value(s')
+    {
+        var new_sent_block_shares := s'.block_share_network.allMessagesSent - s.block_share_network.allMessagesSent;
+
+        forall hn, block_share |
+                && hn in s'.honest_nodes_states.Keys
+                && block_share in s'.block_share_network.allMessagesSent
+                && var block_signing_root := compute_block_signing_root(block_share.block);
+                && verify_bls_signature(block_signing_root, block_share.signature, hn)
+        ensures s'.consensus_instances_on_beacon_block[block_share.block.slot].decided_value.isPresent();
+        ensures s'.consensus_instances_on_beacon_block[block_share.block.slot].decided_value.safe_get() == block_share.block;
+        {
+            var block_signing_root := compute_block_signing_root(block_share.block);
+
+            if block_share in s.block_share_network.allMessagesSent
+            {
+                assert s.consensus_instances_on_beacon_block[block_share.block.slot].decided_value.isPresent();
+                assert s.consensus_instances_on_beacon_block[block_share.block.slot].decided_value.safe_get() == block_share.block;
+            }
+            else
+            {
+                forall signer | verify_bls_signature(block_signing_root, block_share.signature, signer)
+                ensures signer in s.adversary.nodes;
+                ensures signer !in  s.honest_nodes_states.Keys;
+                {
+
+                    assert signer in s.adversary.nodes;
+                    lemmaEmptyIntersectionImpliesDisjointness(s.adversary.nodes, s.honest_nodes_states.Keys);
+                    assert s.adversary.nodes !! s.honest_nodes_states.Keys;
+                    assert signer !in  s.honest_nodes_states.Keys;
+                }
+                assert false;
+            }
+        }
+
+        assert inv_block_of_in_transit_block_share_is_decided_value(s');
+    }
+
+
+    lemma lem_inv_block_of_in_transit_block_share_is_decided_value_dv_next(
+        s: DVState,
+        event: DV_Block_Proposer_Spec.Event,
+        s': DVState
+    )
+    requires NextEventPreCond(s, event)
+    requires NextEvent(s, event, s')
+    requires inv_quorum_constraints(s)
+    requires inv_unchanged_paras_of_consensus_instances(s)
+    requires inv_same_node_status_in_dv_and_ci(s)
+    requires inv_only_dv_construct_complete_signing_functions(s)
+    requires inv_block_of_in_transit_block_share_is_decided_value(s)
+    requires inv_decided_value_of_consensus_instance_of_slot_k_is_for_slot_k(s)
+    requires inv_block_shares_to_broadcast_is_a_subset_of_all_sent_messages(s)
+    requires inv_decided_value_of_consensus_instance_is_decided_by_quorum(s)
+    requires inv_sent_validity_predicate_is_based_on_rcvd_proposer_duty_and_slashing_db_and_randao_reveal(s)
+    requires inv_sent_validity_predicate_is_based_on_rcvd_proposer_duty_and_slashing_db_and_randao_reveal_for_dv(s)
+    ensures inv_block_of_in_transit_block_share_is_decided_value(s')
+    {
+        match event
+        {
+            case HonestNodeTakingStep(node, nodeEvent, nodeOutputs) =>
+                var dvc := s.honest_nodes_states[node];
+                var dvc' := s'.honest_nodes_states[node];
+                match nodeEvent
+                {
+                    case ServeProposerDuty(proposer_duty) =>     
+                        lem_inv_block_of_in_transit_block_share_is_decided_value_dv_next_ServeProposerDuty(s, event, s');
+
+                    case ReceiveRandaoShare(randao_share) =>        
+                        lem_inv_block_of_in_transit_block_share_is_decided_value_dv_next_ReceiveRandaoShare(s, event, s');  
+                        
+                    case BlockConsensusDecided(id, decided_beacon_block) => 
+                        if f_block_consensus_decided.requires(dvc, id, decided_beacon_block)
+                        {
+                            lem_inv_block_of_in_transit_block_share_is_decided_value_BlockConsensusDecided(s, event, s');        
+                        }                 
+                        
+                    case ReceiveSignedBeaconBlock(block_share) =>             
+                        lem_inv_block_of_in_transit_block_share_is_decided_value_dv_next_ReceiveSignedBeaconBlock(s, event, s');           
    
                     case ImportedNewBlock(block) => 
-                        assert inv_unique_rcvd_att_duty_per_slot(dv');     
-                                          
-                    case ResendAttestationShares =>  
-                        assert inv_unique_rcvd_att_duty_per_slot(dv');     
+                        lem_inv_block_of_in_transit_block_share_is_decided_value_dv_next_ImportedNewBlock(s, event, s');           
 
+                    case ResendRandaoRevealSignatureShare =>
+                        lem_inv_block_of_in_transit_block_share_is_decided_value_when_no_new_block_share_is_added(s, event, s');
+
+                    case ResendBlockShare =>
+                        lem_inv_block_of_in_transit_block_share_is_decided_value_dv_next_ResendBlockShare(s, event, s');
+                        
                     case NoEvent => 
-                        assert dvc == dvc'; 
-                        assert dvc.all_rcvd_duties == dvc'.all_rcvd_duties;  
-                        assert inv_unique_rcvd_att_duty_per_slot(dv'); 
+                        assert s'.block_share_network == s.block_share_network;
+                        lem_inv_block_of_in_transit_block_share_is_decided_value_when_no_new_block_share_is_added(s, event, s');
                 }
 
-            case AdversaryTakingStep(node, new_attestation_shares_sent, messagesReceivedByTheNode) =>
-                assert inv_unique_rcvd_att_duty_per_slot(dv');        
+            case AdversaryTakingStep(node, new_randao_shares_sent, new_sent_block_shares, randaoShareReceivedByTheNode, blockShareReceivedByTheNode) =>
+                lem_inv_block_of_in_transit_block_share_is_decided_value_proposer_adversary(s, event, s');
+        }
+    }
+
+    lemma lem_inv_decided_value_of_consensus_instance_of_slot_k_is_for_slot_k_dv_next(
+        s: DVState,
+        event: DV_Block_Proposer_Spec.Event,
+        s': DVState
+    )
+    requires NextEventPreCond(s, event)
+    requires NextEvent(s, event, s')
+    requires inv_quorum_constraints(s)
+    requires inv_unchanged_paras_of_consensus_instances(s)    
+    requires inv_only_dv_construct_complete_signing_functions(s)
+    requires inv_decided_value_of_consensus_instance_is_decided_by_quorum(s)
+    requires inv_sent_validity_predicate_is_based_on_rcvd_proposer_duty_and_slashing_db_and_randao_reveal(s)
+    requires inv_sent_validity_predicate_is_based_on_rcvd_proposer_duty_and_slashing_db_and_randao_reveal_for_dv(s)
+    ensures inv_decided_value_of_consensus_instance_of_slot_k_is_for_slot_k(s')
+    {
+        lem_inv_quorum_constraints_dv_next(s, event, s');
+        lem_inv_unchanged_paras_of_consensus_instances_dv_next(s, event, s');
+        lem_inv_only_dv_construct_complete_signing_functions_dv_next(s, event, s');
+        assert inv_only_dv_construct_complete_signed_block(s');
+        lem_inv_decided_value_of_consensus_instance_is_decided_by_quorum_dv_next(s, event, s');
+        lem_inv_sent_validity_predicate_is_based_on_rcvd_proposer_duty_and_slashing_db_and_randao_reveal_dv_next(s, event, s');
+        lem_inv_decided_value_of_consensus_instance_of_slot_k_is_for_slot_k2(s');
+    }
+
+    lemma lem_inv_block_slashing_db_hist_keeps_track_of_only_rcvd_proposer_duties_dv_next(
+        dv: DVState,
+        event: DV_Block_Proposer_Spec.Event,
+        dv': DVState
+    )    
+    requires NextEventPreCond(dv, event)
+    requires NextEvent(dv, event, dv')    
+    requires inv_consensus_instance_only_for_slot_in_which_dvc_has_rcvd_proposer_duty(dv)
+    requires inv_current_proposer_duty_is_rcvd_duty(dv)
+    requires inv_active_consensus_instances_on_beacon_blocks_are_tracked_in_block_slashing_db_hist(dv)
+    requires inv_block_slashing_db_hist_keeps_track_of_only_rcvd_proposer_duties(dv)  
+    ensures inv_block_slashing_db_hist_keeps_track_of_only_rcvd_proposer_duties(dv')
+    {        
+        match event 
+        {
+            case HonestNodeTakingStep(node, nodeEvent, nodeOutputs) =>
+                var dvc := dv.honest_nodes_states[node];
+                var dvc' := dv'.honest_nodes_states[node];                
+                
+                match nodeEvent
+                {
+                    case ServeProposerDuty(proposer_duty) =>   
+                        assert inv_consensus_instance_only_for_slot_in_which_dvc_has_rcvd_proposer_duty_body(dvc);   
+                        assert inv_block_slashing_db_hist_keeps_track_of_only_rcvd_proposer_duties_body(dvc);                                           
+                        lem_inv_block_slashing_db_hist_keeps_track_of_only_rcvd_proposer_duties_body_f_serve_proposer_duty(dvc, proposer_duty, dvc');
+                        assert inv_block_slashing_db_hist_keeps_track_of_only_rcvd_proposer_duties_body(dvc');
+
+                    case ReceiveRandaoShare(randao_share) =>                         
+                        lem_inv_block_slashing_db_hist_keeps_track_of_only_rcvd_proposer_duties_body_f_listen_for_randao_shares(dvc, randao_share, dvc');    
+                        assert inv_block_slashing_db_hist_keeps_track_of_only_rcvd_proposer_duties_body(dvc');                        
+
+                    case BlockConsensusDecided(id, decided_beacon_block) => 
+                        if f_block_consensus_decided.requires(dvc, id, decided_beacon_block)
+                        {
+                            lem_inv_block_slashing_db_hist_keeps_track_of_only_rcvd_proposer_duties_body_f_block_consensus_decided(dvc, id, decided_beacon_block, dvc');
+                            assert inv_block_slashing_db_hist_keeps_track_of_only_rcvd_proposer_duties_body(dvc');
+                        }
+                        
+                    case ReceiveSignedBeaconBlock(block_share) =>                         
+                        lem_inv_block_slashing_db_hist_keeps_track_of_only_rcvd_proposer_duties_body_f_listen_for_block_signature_shares(dvc, block_share, dvc');
+                        assert inv_block_slashing_db_hist_keeps_track_of_only_rcvd_proposer_duties_body(dvc');
+                       
+                    case ImportedNewBlock(block) => 
+                        var dvc_mod := f_add_block_to_bn(dvc, block);
+                        lem_inv_block_slashing_db_hist_keeps_track_of_only_rcvd_proposer_duties_body_f_add_block_to_bn(dvc, block, dvc_mod);
+                        assert inv_block_slashing_db_hist_keeps_track_of_only_rcvd_proposer_duties_body(dvc_mod);
+                        lem_inv_block_slashing_db_hist_keeps_track_of_only_rcvd_proposer_duties_body_f_listen_for_new_imported_blocks(dvc_mod, block, dvc');                        
+                        assert inv_block_slashing_db_hist_keeps_track_of_only_rcvd_proposer_duties_body(dvc');
+
+                    case ResendBlockShare =>      
+
+                    case ResendRandaoRevealSignatureShare =>                                                                
+
+                    case NoEvent => 
+                        
+                }
+                
+            case AdversaryTakingStep(node, new_randao_shares_sent, new_sent_block_shares, randaoShareReceivedByTheNode, blockShareReceivedByTheNode) =>
                 
         }   
     }
 
-    // lemma lem_inv_slot_of_active_consensus_instance_is_not_higher_than_slot_of_latest_served_proposer_duty_dv_next(
-    //     dv: DVState,
-    //     event: DV_Block_Proposer_Spec.Event,
-    //     dv': DVState
-    // )    
-    // requires NextEventPreCond(dv, event)
-    // requires NextEvent(dv, event, dv')    
-    // requires inv_latest_served_duty_is_rcvd_duty(dv)
-    // requires inv_is_sequence_proposer_duties_to_be_serves_orders(dv)
-    // requires inv_proposer_duty_in_next_delivery_is_not_lower_than_rcvd_proposer_duties(dv)
-    // requires inv_no_active_consensus_instance_before_receiving_a_proposer_duty(dv)
-    // requires inv_slot_of_active_consensus_instance_is_not_higher_than_slot_of_latest_served_proposer_duty(dv)  
-    // ensures inv_slot_of_active_consensus_instance_is_not_higher_than_slot_of_latest_served_proposer_duty(dv')
-    // {        
-    //     match event 
-    //     {
-    //         case HonestNodeTakingStep(node, nodeEvent, nodeOutputs) =>
-    //             var dvc := dv.honest_nodes_states[node];
-    //             var dvc' := dv'.honest_nodes_states[node];                
-                
-    //             match nodeEvent
-    //             {
-    //                 case ServeProposerDuty(proposer_duty) =>   
-    //                     assert inv_latest_served_duty_is_rcvd_duty_body(dvc);                
-    //                     assert inv_proposer_duty_in_next_delivery_is_not_lower_than_rcvd_proposer_duties_body(dvc, proposer_duty);
-    //                     assert inv_no_active_consensus_instance_before_receiving_a_proposer_duty_body(dvc);
-    //                     assert inv_slot_of_active_consensus_instance_is_not_higher_than_slot_of_latest_served_proposer_duty_body(dvc);                                           
-    //                     lem_inv_slot_of_active_consensus_instance_is_not_higher_than_slot_of_latest_served_proposer_duty_body_f_serve_proposer_duty(dvc, proposer_duty, dvc');
-    //                     assert inv_slot_of_active_consensus_instance_is_not_higher_than_slot_of_latest_served_proposer_duty_body(dvc');
+    lemma lem_inv_exists_db_in_block_slashing_db_hist_and_proposer_duty_and_randao_reveal_for_every_validity_predicate_dv_next(
+        dv: DVState,
+        event: DV_Block_Proposer_Spec.Event,
+        dv': DVState
+    )    
+    requires NextEventPreCond(dv, event)
+    requires NextEvent(dv, event, dv')  
+    requires inv_consensus_instances_only_for_rcvd_duties(dv)
+    requires inv_exists_db_in_block_slashing_db_hist_and_proposer_duty_and_randao_reveal_for_every_validity_predicate(dv)
+    ensures inv_exists_db_in_block_slashing_db_hist_and_proposer_duty_and_randao_reveal_for_every_validity_predicate(dv')
+    {        
+        match event 
+        {
+            case HonestNodeTakingStep(node, nodeEvent, nodeOutputs) =>
+                var dvc := dv.honest_nodes_states[node];
+                var dvc' := dv'.honest_nodes_states[node];
+                match nodeEvent
+                {
+                    case ServeProposerDuty(proposer_duty) =>     
+                        lem_inv_exists_db_in_block_slashing_db_hist_and_proposer_duty_and_randao_reveal_for_every_validity_predicate_body_f_serve_proposer_duty(dvc, proposer_duty, dvc');
+                    
+                    case ReceiveRandaoShare(randao_share) =>                         
+                        lem_inv_exists_db_in_block_slashing_db_hist_and_proposer_duty_and_randao_reveal_for_every_validity_predicate_body_f_listen_for_randao_shares(dvc, randao_share, dvc');    
                         
-    //                 case BlockConsensusDecided(id, decided_beacon_block) => 
-    //                     if f_block_consensus_decided.requires(dvc, id, decided_beacon_block)
-    //                     {
-    //                         assert inv_no_active_consensus_instance_before_receiving_a_proposer_duty_body(dvc);
-    //                         lem_inv_slot_of_active_consensus_instance_is_not_higher_than_slot_of_latest_served_proposer_duty_body_f_block_consensus_decided(dvc, id, decided_beacon_block, dvc');
-    //                         assert inv_slot_of_active_consensus_instance_is_not_higher_than_slot_of_latest_served_proposer_duty_body(dvc');
-    //                     }
+                    case BlockConsensusDecided(id, decided_beacon_block) => 
+                        if f_block_consensus_decided.requires(dvc, id, decided_beacon_block)
+                        {
+                            lem_inv_exists_db_in_block_slashing_db_hist_and_proposer_duty_and_randao_reveal_for_every_validity_predicate_body_f_block_consensus_decided(dvc, id, decided_beacon_block, dvc');      
+                        }                 
+                        
+                    case ReceiveSignedBeaconBlock(block_share) =>                         
+                        lem_inv_exists_db_in_block_slashing_db_hist_and_proposer_duty_and_randao_reveal_for_every_validity_predicate_body_f_listen_for_block_signature_shares(dvc, block_share, dvc');                        
+   
+                    case ImportedNewBlock(block) => 
+                        var dvc := f_add_block_to_bn(dvc, nodeEvent.block);
+                        lem_inv_exists_db_in_block_slashing_db_hist_and_proposer_duty_and_randao_reveal_for_every_validity_predicate_body_f_listen_for_new_imported_blocks(dvc, block, dvc');                        
+                                                
+                    case ResendRandaoRevealSignatureShare =>
 
-    //                 case ReceiveRandaoShare(randao_share) =>                         
-    //                     lem_inv_slot_of_active_consensus_instance_is_not_higher_than_slot_of_latest_served_proposer_duty_body_f_listen_for_randao_shares(dvc, randao_share, dvc');
-    //                     assert inv_slot_of_active_consensus_instance_is_not_higher_than_slot_of_latest_served_proposer_duty_body(dvc');
+                    case ResendBlockShare =>
+                        
+                    case NoEvent => 
+                        
+                }
+
+            case AdversaryTakingStep(node, new_randao_shares_sent, new_sent_block_shares, randaoShareReceivedByTheNode, blockShareReceivedByTheNode) =>
+                
+        }   
+    } 
+
+    lemma lem_inv_current_validity_predicate_for_slot_k_is_stored_in_block_slashing_db_hist_k_dv_next(
+        dv: DVState,
+        event: DV_Block_Proposer_Spec.Event,
+        dv': DVState
+    )    
+    requires NextEventPreCond(dv, event)
+    requires NextEvent(dv, event, dv')  
+    requires inv_current_validity_predicate_for_slot_k_is_stored_in_block_slashing_db_hist_k(dv)
+    ensures inv_current_validity_predicate_for_slot_k_is_stored_in_block_slashing_db_hist_k(dv')
+    {        
+        match event 
+        {
+            case HonestNodeTakingStep(node, nodeEvent, nodeOutputs) =>
+                var dvc := dv.honest_nodes_states[node];
+                var dvc' := dv'.honest_nodes_states[node];
+                match nodeEvent
+                {
+                    case ServeProposerDuty(proposer_duty) =>     
+                        lem_inv_current_validity_predicate_for_slot_k_is_stored_in_block_slashing_db_hist_k_body_f_serve_proposer_duty(dvc, proposer_duty, dvc');
+                    
+                    case ReceiveRandaoShare(randao_share) =>                         
+                        lem_inv_current_validity_predicate_for_slot_k_is_stored_in_block_slashing_db_hist_k_body_f_listen_for_randao_shares(dvc, randao_share, dvc');    
+                        
+                    case BlockConsensusDecided(id, decided_beacon_block) => 
+                        if f_block_consensus_decided.requires(dvc, id, decided_beacon_block)
+                        {
+                            lem_inv_current_validity_predicate_for_slot_k_is_stored_in_block_slashing_db_hist_k_body_f_block_consensus_decided(dvc, id, decided_beacon_block, dvc');      
+                        }                 
+                        
+                    case ReceiveSignedBeaconBlock(block_share) =>                         
+                        lem_inv_current_validity_predicate_for_slot_k_is_stored_in_block_slashing_db_hist_k_body_f_listen_for_block_signature_shares(dvc, block_share, dvc');                        
+   
+                    case ImportedNewBlock(block) => 
+                        var dvc := f_add_block_to_bn(dvc, nodeEvent.block);
+                        lem_inv_current_validity_predicate_for_slot_k_is_stored_in_block_slashing_db_hist_k_body_f_listen_for_new_imported_blocks(dvc, block, dvc');                        
+                                                
+                    case ResendRandaoRevealSignatureShare =>
+
+                    case ResendBlockShare =>
+                        
+                    case NoEvent => 
+                        
+                }
+
+            case AdversaryTakingStep(node, new_randao_shares_sent, new_sent_block_shares, randaoShareReceivedByTheNode, blockShareReceivedByTheNode) =>
+                
+        }   
+    } 
+
+    lemma lem_inv_monotonic_block_slashing_db_hist_dv_next(
+        dv: DVState,
+        event: DV_Block_Proposer_Spec.Event,
+        dv': DVState
+    )    
+    requires NextEventPreCond(dv, event)
+    requires NextEvent(dv, event, dv')  
+    ensures inv_monotonic_block_slashing_db_hist(dv, event, dv')
+    {        
+        match event 
+        {
+            case HonestNodeTakingStep(node, nodeEvent, nodeOutputs) =>
+                var dvc := dv.honest_nodes_states[node];
+                var dvc' := dv'.honest_nodes_states[node];
+                match nodeEvent
+                {
+                    case ServeProposerDuty(proposer_duty) =>     
+                        lem_inv_block_slashing_db_hist_is_monotonic_dvc_f_serve_proposer_duty(dvc, proposer_duty, dvc');
+                    
+                    case ReceiveRandaoShare(randao_share) =>                         
+                        lem_inv_block_slashing_db_hist_is_monotonic_dvc_f_listen_for_randao_shares(dvc, randao_share, dvc');    
+                        
+                    case BlockConsensusDecided(id, decided_beacon_block) => 
+                        if f_block_consensus_decided.requires(dvc, id, decided_beacon_block)
+                        {
+                            lem_inv_block_slashing_db_hist_is_monotonic_dvc_f_block_consensus_decided(dvc, id, decided_beacon_block, dvc');      
+                        }                 
+                        
+                    case ReceiveSignedBeaconBlock(block_share) =>                         
+                        lem_inv_block_slashing_db_hist_is_monotonic_dvc_f_listen_for_block_signature_shares(dvc, block_share, dvc');                        
+   
+                    case ImportedNewBlock(block) => 
+                        var dvc := f_add_block_to_bn(dvc, nodeEvent.block);
+                        lem_inv_block_slashing_db_hist_is_monotonic_dvc_f_listen_for_new_imported_blocks(dvc, block, dvc');                        
+                                                
+                    case ResendRandaoRevealSignatureShare =>
+
+                    case ResendBlockShare =>
+                        
+                    case NoEvent => 
+                        
+                }
+
+            case AdversaryTakingStep(node, new_randao_shares_sent, new_sent_block_shares, randaoShareReceivedByTheNode, blockShareReceivedByTheNode) =>
+                
+        }   
+    } 
+
+
+    lemma lem_inv_every_db_in_block_slashing_db_hist_is_subset_of_block_slashing_db_dv_next(
+        dv: DVState,
+        event: DV_Block_Proposer_Spec.Event,
+        dv': DVState
+    )    
+    requires NextEventPreCond(dv, event)
+    requires NextEvent(dv, event, dv')    
+    requires inv_consensus_instances_only_for_rcvd_duties(dv)
+    requires inv_every_db_in_block_slashing_db_hist_is_subset_of_block_slashing_db(dv)  
+    ensures inv_every_db_in_block_slashing_db_hist_is_subset_of_block_slashing_db(dv')
+    {        
+        match event 
+        {
+            case HonestNodeTakingStep(node, nodeEvent, nodeOutputs) =>
+                var dvc := dv.honest_nodes_states[node];
+                var dvc' := dv'.honest_nodes_states[node];                
+                
+                match nodeEvent
+                {
+                    case ServeProposerDuty(proposer_duty) =>   
+                        assert inv_consensus_instances_only_for_rcvd_duties_body(dvc);   
+                        assert inv_every_db_in_block_slashing_db_hist_is_subset_of_block_slashing_db_body(dvc);                                           
+                        lem_inv_every_db_in_block_slashing_db_hist_is_subset_of_block_slashing_db_body_f_serve_proposer_duty(dvc, proposer_duty, dvc');
+                        assert inv_every_db_in_block_slashing_db_hist_is_subset_of_block_slashing_db_body(dvc');
+
+                    case ReceiveRandaoShare(randao_share) =>        
+                        lem_inv_every_db_in_block_slashing_db_hist_is_subset_of_block_slashing_db_body_f_listen_for_randao_shares(dvc, randao_share, dvc');   
+                        assert inv_every_db_in_block_slashing_db_hist_is_subset_of_block_slashing_db_body(dvc');                        
+
+                    case BlockConsensusDecided(id, decided_beacon_block) => 
+                        lem_inv_every_db_in_block_slashing_db_hist_is_subset_of_block_slashing_db_body_f_block_consensus_decided(dvc, id, decided_beacon_block, dvc');
+                        assert inv_every_db_in_block_slashing_db_hist_is_subset_of_block_slashing_db_body(dvc');
+                        
+                    case ReceiveSignedBeaconBlock(block_share) =>                         
+                        lem_inv_every_db_in_block_slashing_db_hist_is_subset_of_block_slashing_db_body_f_listen_for_block_signature_shares(dvc, block_share, dvc');
+                        assert inv_every_db_in_block_slashing_db_hist_is_subset_of_block_slashing_db_body(dvc');
                        
-    //                 case ImportedNewBlock(block) => 
-    //                     assert inv_no_active_consensus_instance_before_receiving_a_proposer_duty_body(dvc);
-                        
-    //                     var dvc_mod := f_add_block_to_bn(dvc, block);
-    //                     lem_inv_no_active_consensus_instance_before_receiving_a_proposer_duty_body_f_add_block_to_bn(dvc, block, dvc_mod);
-    //                     assert inv_no_active_consensus_instance_before_receiving_a_proposer_duty_body(dvc_mod);
-    //                     lem_inv_slot_of_active_consensus_instance_is_not_higher_than_slot_of_latest_served_proposer_duty_body_f_add_block_to_bn(dvc, block, dvc_mod);
-    //                     assert inv_slot_of_active_consensus_instance_is_not_higher_than_slot_of_latest_served_proposer_duty_body(dvc_mod);
-    //                     lem_inv_slot_of_active_consensus_instance_is_not_higher_than_slot_of_latest_served_proposer_duty_body_f_listen_for_new_imported_blocks(dvc_mod, block, dvc');                        
-    //                     assert inv_slot_of_active_consensus_instance_is_not_higher_than_slot_of_latest_served_proposer_duty_body(dvc');
+                    case ImportedNewBlock(block) => 
+                        var dvc_mod := f_add_block_to_bn(dvc, block);
+                        lem_inv_every_db_in_block_slashing_db_hist_is_subset_of_block_slashing_db_body_f_add_block_to_bn(dvc, block, dvc_mod);
+                        assert inv_every_db_in_block_slashing_db_hist_is_subset_of_block_slashing_db_body(dvc_mod);
+                        lem_inv_every_db_in_block_slashing_db_hist_is_subset_of_block_slashing_db_body_f_listen_for_new_imported_blocks(dvc_mod, block, dvc');                        
+                        assert inv_every_db_in_block_slashing_db_hist_is_subset_of_block_slashing_db_body(dvc');
 
-    //                 case ResendRandaoRevealSignatureShare =>                                                                      
+                    case ResendRandaoRevealSignatureShare =>
+                        assert inv_every_db_in_block_slashing_db_hist_is_subset_of_block_slashing_db_body(dvc');
+                    
+                    case ResendBlockShare =>                                                                    
+                        assert inv_every_db_in_block_slashing_db_hist_is_subset_of_block_slashing_db_body(dvc');  
 
-    //                 case NoEvent => 
+                    case NoEvent => 
+                        assert inv_every_db_in_block_slashing_db_hist_is_subset_of_block_slashing_db_body(dvc');
                         
-    //             }
+                }
                 
-    //         case AdversaryTakingStep(node, new_randao_shares_sent, messagesReceivedByTheNode) =>
+            case AdversaryTakingStep(node, new_randao_shares_sent, new_sent_block_shares, randaoShareReceivedByTheNode, blockShareReceivedByTheNode) =>
+                assert inv_every_db_in_block_slashing_db_hist_is_subset_of_block_slashing_db(dv');
                 
-    //     }   
-    // } 
+        }   
+    }
+
+      
+
+    lemma lem_inv_sent_validity_predicate_is_based_on_rcvd_proposer_duty_and_slashing_db_and_randao_reveal_for_dv_dv_next(
+        s: DVState,
+        event: DV_Block_Proposer_Spec.Event,
+        s': DVState
+    )
+    requires NextEventPreCond(s, event)
+    requires NextEvent(s, event, s')
+    requires inv_quorum_constraints(s)
+    requires inv_unchanged_paras_of_consensus_instances(s)
+    requires inv_only_dv_construct_complete_signed_block(s)
+    requires inv_consensus_instances_only_for_rcvd_duties(s)
+    requires inv_exists_db_in_block_slashing_db_hist_and_proposer_duty_and_randao_reveal_for_every_validity_predicate(s)    
+    requires inv_sent_validity_predicate_is_based_on_rcvd_proposer_duty_and_slashing_db_and_randao_reveal_for_dv(s)
+    ensures inv_sent_validity_predicate_is_based_on_rcvd_proposer_duty_and_slashing_db_and_randao_reveal_for_dv(s')
+    {
+        match event
+        {
+            case HonestNodeTakingStep(node, nodeEvent, nodeOutputs) =>
+                var dvc := s.honest_nodes_states[node];
+                var dvc' := s'.honest_nodes_states[node];
+                match nodeEvent
+                {
+                    case ServeProposerDuty(proposer_duty) =>
+                        lem_inv_sent_validity_predicate_is_based_on_rcvd_proposer_duty_and_slashing_db_and_randao_reveal_for_dvc_f_serve_proposer_duty(dvc, proposer_duty, dvc');
+
+                    case ReceiveRandaoShare(randao_share) =>                         
+                        lem_inv_sent_validity_predicate_is_based_on_rcvd_proposer_duty_and_slashing_db_and_randao_reveal_for_dvc_f_listen_for_randao_shares(dvc, randao_share, dvc');
+
+                    case BlockConsensusDecided(id, decided_beacon_block) =>
+                        if f_block_consensus_decided.requires(dvc, id, decided_beacon_block)
+                        {
+                            lem_inv_sent_validity_predicate_is_based_on_rcvd_proposer_duty_and_slashing_db_and_randao_reveal_for_dvc_f_block_consensus_decided(dvc, id, decided_beacon_block, dvc');      
+                        }   
+
+                    case ReceiveSignedBeaconBlock(block_share) =>
+                        lem_inv_sent_validity_predicate_is_based_on_rcvd_proposer_duty_and_slashing_db_and_randao_reveal_for_dvc_f_listen_for_block_signature_shares(dvc, block_share, dvc');
+
+                    case ImportedNewBlock(block) =>
+                        var dvc_after_adding_new_block := f_add_block_to_bn(dvc, nodeEvent.block);
+                        lem_inv_sent_validity_predicate_is_based_on_rcvd_proposer_duty_and_slashing_db_and_randao_reveal_for_dvc_f_add_block_to_bn(
+                            dvc,
+                            block,
+                            dvc_after_adding_new_block
+                        );
+                        lem_inv_sent_validity_predicate_is_based_on_rcvd_proposer_duty_and_slashing_db_and_randao_reveal_for_dvc_f_listen_for_new_imported_blocks(
+                            dvc_after_adding_new_block, 
+                            block, 
+                            dvc'
+                        );                            
+
+                    case ResendRandaoRevealSignatureShare =>
+                        lem_inv_sent_validity_predicate_is_based_on_rcvd_proposer_duty_and_slashing_db_and_randao_reveal_for_dvc_f_resend_randao_share(dvc, dvc');
+
+                    case ResendBlockShare =>
+                        lem_inv_sent_validity_predicate_is_based_on_rcvd_proposer_duty_and_slashing_db_and_randao_reveal_for_dvc_f_resend_block_share(dvc, dvc');
+
+                    case NoEvent =>
+                        assert dvc == dvc';
+
+                }
+
+            case AdversaryTakingStep(node, new_randao_shares_sent, new_sent_block_shares, randaoShareReceivedByTheNode, blockShareReceivedByTheNode) =>
+                assert inv_sent_validity_predicate_is_based_on_rcvd_proposer_duty_and_slashing_db_and_randao_reveal_for_dv(s');
+        }
+    }
 }   
         
